@prefix : <http://purl.org/ai4st/ontology#> .
@prefix owl: <http://www.w3.org/2002/07/owl#> .
@prefix rdf: <http://www.w3.org/1999/02/22-rdf-syntax-ns#> .
@prefix xml: <http://www.w3.org/XML/1998/namespace> .
@prefix xsd: <http://www.w3.org/2001/XMLSchema#> .
@prefix rdfs: <http://www.w3.org/2000/01/rdf-schema#> .
@base <http://purl.org/ai4st/ontology#> .

<http://purl.org/ai4st/ontology#> rdf:type owl:Ontology ;
                                   owl:versionIRI <http://purl.org/ai4st/ontology#/1.0.0> ;
                                   owl:imports <http://purl.org/stc/ontology#/1.0.0> ;
                                   <http://purl.org/dc/elements/1.1/creator> "Schieferdecker, Ina K." ;
                                   <http://purl.org/dc/elements/1.1/title> "ai4st: The AI for ST taxonomy"@en ;
                                   <http://purl.org/dc/terms/bibliographicCitation> "Schieferdecker, I.K.: \"ai4st: A taxonomy of research papers on the support of software testing (ST) through the use of artificial intelligence (AI) methods and techniques\", 2025, http://purl.org/ai4st"@en ;
                                   <http://purl.org/dc/terms/license> "http://creativecommons.org/licenses/by/4.0/legalcode.en" ;
                                   <http://purl.org/vocab/vann/preferredNamespacePrefix> "ai4st:"@en ;
                                   <http://purl.org/vocab/vann/preferredNamespaceUri> "http://purl.org/ai4st/ontology" ;
                                   rdfs:comment "ai4st is a taxonomy for research papers on the use of artificial intelligence (AI) methods and techniques to support software testing (ST).  It relates papers to their topics and contributions. These contributions are categorised by the purpose of the solution aimed for, the ST activity or process targeted, the type of AI used and the level of automation supported."@en ;
                                   owl:versionInfo 1 .

#################################################################
#    Annotation properties
#################################################################

###  http://purl.org/dc/elements/1.1/creator
<http://purl.org/dc/elements/1.1/creator> rdf:type owl:AnnotationProperty .


###  http://purl.org/dc/elements/1.1/title
<http://purl.org/dc/elements/1.1/title> rdf:type owl:AnnotationProperty .


###  http://purl.org/dc/terms/bibliographicCitation
<http://purl.org/dc/terms/bibliographicCitation> rdf:type owl:AnnotationProperty .


###  http://purl.org/dc/terms/license
<http://purl.org/dc/terms/license> rdf:type owl:AnnotationProperty .


###  http://purl.org/vocab/vann/preferredNamespacePrefix
<http://purl.org/vocab/vann/preferredNamespacePrefix> rdf:type owl:AnnotationProperty .


###  http://purl.org/vocab/vann/preferredNamespaceUri
<http://purl.org/vocab/vann/preferredNamespaceUri> rdf:type owl:AnnotationProperty .


#################################################################
#    Object Properties
#################################################################

###  http://purl.org/ai4st/ontology#belongsTo
:belongsTo rdf:type owl:ObjectProperty ,
                    owl:AsymmetricProperty ,
                    owl:TransitiveProperty ,
                    owl:IrreflexiveProperty ;
           rdfs:domain <http://purl.org/nemo/gufo#AbstractIndividualType> ;
           rdfs:range <http://purl.org/nemo/gufo#AbstractIndividualType> .


###  http://purl.org/ai4st/ontology#belongsToAIType
:belongsToAIType rdf:type owl:ObjectProperty ;
                 rdfs:subPropertyOf :belongsTo ;
                 rdf:type owl:TransitiveProperty ;
                 rdfs:domain :AIType ;
                 rdfs:range :AIType .


###  http://purl.org/ai4st/ontology#hasLevel
:hasLevel rdf:type owl:ObjectProperty ;
          rdfs:subPropertyOf <http://purl.org/nemo/gufo#hasAssociatedQualityValueType> ;
          owl:inverseOf :levelEnabledBy ;
          rdfs:domain :ResearchPaper ;
          rdfs:range :AutomationLevel .


###  http://purl.org/ai4st/ontology#hasParent
:hasParent rdf:type owl:ObjectProperty .


###  http://purl.org/ai4st/ontology#hasPurpose
:hasPurpose rdf:type owl:ObjectProperty ;
            rdfs:subPropertyOf <http://purl.org/nemo/gufo#hasAssociatedQualityValueType> ;
            owl:inverseOf :purposeAdressedBy ;
            rdfs:domain :ResearchPaper ;
            rdfs:range :SolutionPurpose .


###  http://purl.org/ai4st/ontology#hasTarget
:hasTarget rdf:type owl:ObjectProperty ;
           rdfs:subPropertyOf <http://purl.org/nemo/gufo#hasAssociatedQualityValueType> ;
           owl:inverseOf :targetFocussedBy ;
           rdfs:domain :ResearchPaper ;
           rdfs:range :Target .


###  http://purl.org/ai4st/ontology#hasType
:hasType rdf:type owl:ObjectProperty ;
         rdfs:subPropertyOf <http://purl.org/nemo/gufo#hasAssociatedQualityValueType> ;
         owl:inverseOf :typeUsedBy ;
         rdfs:domain :ResearchPaper ;
         rdfs:range :AIType .


###  http://purl.org/ai4st/ontology#implementedIn
:implementedIn rdf:type owl:ObjectProperty ;
               rdfs:domain <http://purl.org/nemo/gufo#AbstractIndividualType> ;
               rdfs:range <http://purl.org/nemo/gufo#EndurantType> .


###  http://purl.org/ai4st/ontology#isAboutResearchTopic
:isAboutResearchTopic rdf:type owl:ObjectProperty ;
                      rdfs:subPropertyOf <http://purl.org/nemo/gufo#hasAssociatedQualityValueType> ;
                      owl:inverseOf :topicAddressedBy ;
                      rdfs:domain :ResearchPaper ;
                      rdfs:comment "Represents the research topics that a research paper contributes to."@en ;
                      rdfs:label "isAboutResearchTopic" .


###  http://purl.org/ai4st/ontology#levelEnabledBy
:levelEnabledBy rdf:type owl:ObjectProperty ;
                rdfs:subPropertyOf :implementedIn ;
                rdfs:domain :AutomationLevel ;
                rdfs:range :ResearchPaper .


###  http://purl.org/ai4st/ontology#purposeAdressedBy
:purposeAdressedBy rdf:type owl:ObjectProperty ;
                   rdfs:subPropertyOf :implementedIn ;
                   rdfs:domain :SolutionPurpose ;
                   rdfs:range :ResearchPaper .


###  http://purl.org/ai4st/ontology#targetFocussedBy
:targetFocussedBy rdf:type owl:ObjectProperty ;
                  rdfs:subPropertyOf :implementedIn ;
                  rdfs:domain :Target ;
                  rdfs:range :ResearchPaper .


###  http://purl.org/ai4st/ontology#topicAddressedBy
:topicAddressedBy rdf:type owl:ObjectProperty ;
                  rdfs:subPropertyOf :implementedIn ;
                  rdfs:range :ResearchPaper .


###  http://purl.org/ai4st/ontology#typeUsedBy
:typeUsedBy rdf:type owl:ObjectProperty ;
            rdfs:subPropertyOf :implementedIn ;
            rdfs:domain :AIType ;
            rdfs:range :ResearchPaper .


###  http://purl.org/nemo/gufo#hasAssociatedQualityValueType
<http://purl.org/nemo/gufo#hasAssociatedQualityValueType> rdf:type owl:ObjectProperty .


###  http://purl.org/nemo/gufo#isEventProperPartOf
<http://purl.org/nemo/gufo#isEventProperPartOf> rdf:type owl:ObjectProperty .


###  http://purl.org/nemo/gufo#mediates
<http://purl.org/nemo/gufo#mediates> rdf:type owl:ObjectProperty .


#################################################################
#    Classes
#################################################################

###  http://purl.org/ai4st/ontology#AIType
:AIType rdf:type owl:Class ;
        rdfs:subClassOf <http://purl.org/nemo/gufo#AbstractIndividualType> ;
        rdfs:comment """Represents the type of the artificial intelligence (AI) system being used.

According to ISO/IEC 22989:2022 Information technology - Artificial intelligence - Artificial intelligence concepts and terminology, artificial intelligence (AI) is

- <discipline> research and development of mechanisms and applications of AI systems.

and

artificial intelligence system (AI system) is

- engineered system that generates outputs such as content, forecasts, recommendations or decisions for a given set of human-defined objectives."""@en ;
        rdfs:label "Type of AI system" .


###  http://purl.org/ai4st/ontology#AutomationLevel
:AutomationLevel rdf:type owl:Class ;
                 rdfs:subClassOf <http://purl.org/nemo/gufo#AbstractIndividualType> ;
                 rdfs:label """Represents the level of automation provided / enabled by the AI system being used.

According to ISO/IEC 22989:2022 Information technology - Artificial intelligence - Artificial intelligence concepts and terminology, artificial intelligence (AI) is

- <discipline> research and development of mechanisms and applications of AI systems.

and

artificial intelligence system (AI system) is

- engineered system that generates outputs such as content, forecasts, recommendations or decisions for a given set of human-defined objectives."""@en ,
                            "Level of AI automation" .


###  http://purl.org/ai4st/ontology#Model
:Model rdf:type owl:Class ;
       rdfs:subClassOf <http://purl.org/nemo/gufo#Mixin> ;
       rdfs:comment """Represents artifacts defining (semi-)formally (1) properties of one or more artefacts used by software engineering activities or processes or (2) properties of software engineering activities or processes.

According to ISO/IEC 22989:2022 Information technology - Artificial intelligence - Artificial intelligence concepts and terminology, model is

- physical, mathematical or otherwise logical representation of a system, entity, phenomenon, process or data.

Note: For the ai4st ontology, only mathematical or logical representations are relevant."""@en ;
       rdfs:label "Model" .


###  http://purl.org/ai4st/ontology#ResearchPaper
:ResearchPaper rdf:type owl:Class ;
               rdfs:subClassOf <http://purl.org/nemo/gufo#Mixin> ;
               rdfs:comment "Represents an artifact documenting research findings like new insights, methods, techniques, etc."@en ;
               rdfs:label "ResearchPaper" .


###  http://purl.org/ai4st/ontology#SolutionPurpose
:SolutionPurpose rdf:type owl:Class ;
                 rdfs:subClassOf <http://purl.org/nemo/gufo#AbstractIndividualType> ;
                 rdfs:comment "Represents the purpose of using the AI system in a software development / operation processes or activities."@en ;
                 rdfs:label "Solution purpose" .


###  http://purl.org/ai4st/ontology#Target
:Target rdf:type owl:Class ;
        rdfs:subClassOf <http://purl.org/nemo/gufo#AbstractIndividualType> ;
        rdfs:comment "Represents the primary concept, issue, component, software, or process in a software engineering process or activitiy being addressed."@en ;
        rdfs:label "Solution target" .


###  http://purl.org/nemo/gufo#AbstractIndividualType
<http://purl.org/nemo/gufo#AbstractIndividualType> rdf:type owl:Class .


###  http://purl.org/nemo/gufo#EndurantType
<http://purl.org/nemo/gufo#EndurantType> rdf:type owl:Class .


###  http://purl.org/nemo/gufo#Mixin
<http://purl.org/nemo/gufo#Mixin> rdf:type owl:Class .


###  https://purl.org/ai4st/ontology#Target
<https://purl.org/ai4st/ontology#Target> rdf:type owl:Class .


#################################################################
#    Individuals
#################################################################

###  http://purl.org/ai4st/new_terms#visual_testing
<http://purl.org/ai4st/new_terms#visual_testing> rdf:type owl:NamedIndividual ,
                                                          <https://purl.org/ai4st/ontology#Target> ;
                                                 :hasParent <http://purl.org/stc/terms#interface_testing> .


###  http://purl.org/ai4st/ontology#AI-assisted_options
:AI-assisted_options rdf:type owl:NamedIndividual ,
                              :AutomationLevel ;
                     rdfs:comment "Represents the case in which choices, recommendations, or decision-support outputs for the target SE processes or activities are generated or enhanced by an AI system, while retaining human control over the final choice, recommendation or decision, which may differ from the AI outputs."@en ;
                     rdfs:label "AI-assisted options" .


###  http://purl.org/ai4st/ontology#AI-assisted_selection
:AI-assisted_selection rdf:type owl:NamedIndividual ,
                                :AutomationLevel ;
                       rdfs:comment "Represents the case in which choices, recommendations, or decision-support outputs for the target SE processes or activities are generated or enhanced by an AI system, where the final choices, recommendations or decisions require human confirmation and do not differ from the AI outputs."@en ;
                       rdfs:label "AI-assisted selection" .


###  http://purl.org/ai4st/ontology#AI-driven_full_automation
:AI-driven_full_automation rdf:type owl:NamedIndividual ,
                                    :AutomationLevel ;
                           rdfs:comment "Represents the case in which AI is used to automate all tasks or decision-making components within the target SE processes or activities, without requiring human intervention."@en ;
                           rdfs:label "AI-driven full automation" .


###  http://purl.org/ai4st/ontology#AI-driven_partial_automation
:AI-driven_partial_automation rdf:type owl:NamedIndividual ,
                                       :AutomationLevel ;
                              rdfs:comment "Represents the case in which AI is used to automate specific tasks or decision-making components within the target SE processes or activities, while other parts of the process remain under human control or require human intervention."@en ;
                              rdfs:label "AI-driven partial automation" .


###  http://purl.org/ai4st/ontology#Agentic_AI
:Agentic_AI rdf:type owl:NamedIndividual ,
                     :AIType ;
            rdfs:comment "Represents AI systems that rely on autonomous agents using AI techniques to plan, adapt, and execute multi-step objectives with minimal human control."@en ;
            rdfs:label "Agentic AI" .


###  http://purl.org/ai4st/ontology#Classical_machine_learning
:Classical_machine_learning rdf:type owl:NamedIndividual ,
                                     :AIType ;
                            :belongsToAIType :Subsymbolic ;
                            rdfs:comment """Represents subsymbolic AI systems that rely on statistical and algorithmic learning techniques - such as decision trees, support vector machines, linear regression, and clustering - to learn patterns from structured data and make predictions or classifications. These models typically operate on explicitly defined features and do not involve deep neural networks.

This class of AI is used in contrast to deep learning AI."""@en ;
                            rdfs:label "Classical machine learning" .


###  http://purl.org/ai4st/ontology#Deep_learning
:Deep_learning rdf:type owl:NamedIndividual ,
                        :AIType ;
               :belongsToAIType :Subsymbolic ;
               rdfs:comment """Represents subsymbolic AI systems that rely on deep artificial neural networks to automatically learn features and perform tasks such as classification or prediction, especially from large and complex datasets. 

According to ISO/IEC 22989:2022 Information technology - Artificial intelligence - Artificial intelligence concepts and terminology, deep learning (deep neural network learning) is

- AI approach to creating rich hierarchical representations through the training of neural networks with many hidden layers."""@en ;
               rdfs:label "Deep learning AI" .


###  http://purl.org/ai4st/ontology#ERP_system
:ERP_system rdf:type owl:NamedIndividual ,
                     <https://purl.org/ai4st/ontology#Target> ;
            :hasParent <http://purl.org/stc/terms#test_object> .


###  http://purl.org/ai4st/ontology#Evolutionary_algorithms
:Evolutionary_algorithms rdf:type owl:NamedIndividual ,
                                  :AIType ;
                         :belongsToAIType :Subsymbolic .


###  http://purl.org/ai4st/ontology#General_AI
:General_AI rdf:type owl:NamedIndividual ,
                     :AIType ;
            rdfs:comment """Represents AI systems capable of performing a broad set of distinct tasks with satisfactory performance.

According to ISO/IEC 22989:2022 Information technology - Artificial intelligence - Artificial intelligence concepts and terminology, general AI (AGI, artificial general intelligence)

- type of AI system that addresses a broad range of tasks with a satisfactory level of performance 

Note 1: Compared to narrow AI.
Note 2: AGI is often used in a stronger sense, meaning systems that not only can perform a wide variety of tasks, but all tasks that a human can perform."""@en ;
            rdfs:label "General AI" .


###  http://purl.org/ai4st/ontology#Generate
:Generate rdf:type owl:NamedIndividual ,
                   :SolutionPurpose .


###  http://purl.org/ai4st/ontology#Generative_AI
:Generative_AI rdf:type owl:NamedIndividual ,
                        :AIType ;
               rdfs:comment "Represents AI systems that use learned or derived knowledge to produce original outputs, such as synthetic text, media, or other content types. It often uses subsymbolic AI like Convolutional Neural Networks (CNNs), Recurrent Neural Networks (RNNs), or Transformer-based models, but also symbolic AI."@en ;
               rdfs:label "Generative AI" .


###  http://purl.org/ai4st/ontology#Improve
:Improve rdf:type owl:NamedIndividual ,
                  :SolutionPurpose ;
         rdfs:comment "The purpose of using AI is to improve (parts of) artefacts used in software engineering."@en ;
         rdfs:label "Improve" .


###  http://purl.org/ai4st/ontology#No_AI_automation
:No_AI_automation rdf:type owl:NamedIndividual ,
                           :AutomationLevel ;
                  rdfs:comment "Represents the case in which the target SE processes or activities are performed without the assistance of AI."@en ;
                  rdfs:label "No AI-supported automation" .


###  http://purl.org/ai4st/ontology#Statistical
:Statistical rdf:type owl:NamedIndividual ,
                      :AIType ;
             :belongsToAIType :Subsymbolic ;
             rdfs:comment "Represents subsymbolic AI systems that rely on data and statistical inference to identify patterns and make predictions."@en ;
             rdfs:label "Statistical AI" .


###  http://purl.org/ai4st/ontology#Subsymbolic
:Subsymbolic rdf:type owl:NamedIndividual ,
                      :AIType ;
             rdfs:comment """Represents AI systems that use numerical models to represent knowledge and computations, such as numerical optimisation and statistical learning, in order to model and solve problems.

According to ISO/IEC 22989:2022 Information technology - Artificial intelligence - Artificial intelligence concepts and terminology, subsymbolic AI is

- AI based on techniques and models that use an implicit encoding of information, that can be derived from experience or raw data."""@en ;
             rdfs:label "Subsymbolic AI" .


###  http://purl.org/ai4st/ontology#Swarm_intelligence
:Swarm_intelligence rdf:type owl:NamedIndividual ,
                             :AIType ;
                    :belongsToAIType :Subsymbolic .


###  http://purl.org/ai4st/ontology#Symbolic
:Symbolic rdf:type owl:NamedIndividual ,
                   :AIType ;
          rdfs:comment """Represents AI systems that use approaches relying on the explicit definition of symbols and rules representing knowledge and performing logical reasoning.

According to ISO/IEC 22989:2022 Information technology - Artificial intelligence - Artificial intelligence concepts and terminology, symbolic AI is

- AI based on techniques and models that manipulate symbols and structures according to explicitly defined rules to obtain inferences."""@en ;
          rdfs:label "Symbolic AI" .


###  http://purl.org/ai4st/ontology#Understand
:Understand rdf:type owl:NamedIndividual ,
                     :SolutionPurpose ;
            rdfs:comment "The purpose of using AI is to gain insight."@en ;
            rdfs:label "Understand" .


###  http://purl.org/ai4st/ontology#Web_application
:Web_application rdf:type owl:NamedIndividual ,
                          <https://purl.org/ai4st/ontology#Target> ;
                 :hasParent <http://purl.org/stc/terms#test_object> .


###  http://purl.org/ai4st/ontology#assertion
:assertion rdf:type owl:NamedIndividual ,
                    <https://purl.org/ai4st/ontology#Target> ;
           :hasParent <http://purl.org/stc/terms#Testware> .


###  http://purl.org/ai4st/ontology#computer_game
:computer_game rdf:type owl:NamedIndividual ,
                        <https://purl.org/ai4st/ontology#Target> ;
               :hasParent <http://purl.org/stc/terms#test_object> .


###  http://purl.org/ai4st/ontology#concolic_testing
:concolic_testing rdf:type owl:NamedIndividual ,
                           <https://purl.org/ai4st/ontology#Target> ;
                  :hasParent <http://purl.org/stc/terms#white_box_test_technique> .


###  http://purl.org/ai4st/ontology#ethics
:ethics rdf:type owl:NamedIndividual ,
                 <https://purl.org/ai4st/ontology#Target> ;
        :hasParent <http://purl.org/stc/terms#basic_concepts> .


###  http://purl.org/ai4st/ontology#mutation_testing
:mutation_testing rdf:type owl:NamedIndividual ,
                           <https://purl.org/ai4st/ontology#Target> ;
                  :hasParent <http://purl.org/stc/terms#white_box_test_technique> .


###  http://purl.org/ai4st/ontology#null
:null rdf:type owl:NamedIndividual ,
               owl:Thing .


###  http://purl.org/ai4st/ontology#penetration_testing
:penetration_testing rdf:type owl:NamedIndividual ,
                              <https://purl.org/ai4st/ontology#Target> ;
                     :hasParent <http://purl.org/stc/terms#security_testing> .


###  http://purl.org/ai4st/ontology#test_documentation
:test_documentation rdf:type owl:NamedIndividual ,
                             <https://purl.org/ai4st/ontology#Target> ;
                    :hasParent <http://purl.org/stc/terms#test_activity> .


###  http://purl.org/ai4st/ontology#test_generation
:test_generation rdf:type owl:NamedIndividual ,
                          <https://purl.org/ai4st/ontology#Target> ;
                 :hasParent <http://purl.org/stc/terms#test_activity> .


###  http://purl.org/ai4st/ontology#test_prioritization
:test_prioritization rdf:type owl:NamedIndividual ,
                              <https://purl.org/ai4st/ontology#Target> ;
                     :hasParent <http://purl.org/stc/terms#test_activity> .


###  http://purl.org/ai4st/ontology#test_selection
:test_selection rdf:type owl:NamedIndividual ,
                         <https://purl.org/ai4st/ontology#Target> ;
                :hasParent <http://purl.org/stc/terms#test_execution> .


###  http://purl.org/ai4st/ontology#test_verification
:test_verification rdf:type owl:NamedIndividual ,
                            <https://purl.org/ai4st/ontology#Target> ;
                   :hasParent <http://purl.org/stc/terms#test_activity> .


###  http://purl.org/ai4st/ontology#CSO:Testing_and_Debugging
:CSO:Testing_and_Debugging rdf:type owl:NamedIndividual .


###  http://purl.org/ai4st/papers#abdelkarim_tcp-net_2023
<http://purl.org/ai4st/papers#abdelkarim_tcp-net_2023> rdf:type owl:NamedIndividual ,
                                                                :ResearchPaper ;
                                                       :hasLevel :AI-assisted_options ;
                                                       :hasPurpose :Generate ;
                                                       :hasTarget :test_prioritization ;
                                                       :hasType :Deep_learning ;
                                                       :isAboutResearchTopic :CSO:Testing_and_Debugging ;
                                                       rdfs:comment """@inproceedings{abdelkarim_tcp-net_2023,
 address = {Athens, Greece},
 author = {Abdelkarim, Mohamed and ElAdawi, Reem},
 booktitle = {2023 {IEEE} {International} {Conference} {On} {Artificial} {Intelligence} {Testing} ({AITest})},
 copyright = {http://doi.org/10.15223/policy-029},
 doi = {10.1109/AITest58265.2023.00024},
 isbn = {979-8-3503-3629-0},
 month = {July},
 pages = {99--106},
 publisher = {IEEE},
 shorttitle = {{TCP}-{Net}++},
 title = {{TCP}-{Net}++: {Test} {Case} {Prioritization} {Using} {End}-to-{End} {Deep} {Neural} {Networks} - {Deployment} {Analysis} and {Enhancements}},
 url = {http://ieeexplore.ieee.org/document/10229439/},
 urldate = {2025-06-12},
 year = {2023}
}
""" ;
                                                       rdfs:label "abdelkarim_tcp-net_2023" ;
                                                       rdfs:seeAlso <http://ieeexplore.ieee.org/document/10229439/> .


###  http://purl.org/ai4st/papers#caglar_development_2023
<http://purl.org/ai4st/papers#caglar_development_2023> rdf:type owl:NamedIndividual ,
                                                                :ResearchPaper ;
                                                       :hasLevel :AI-driven_full_automation ;
                                                       :hasPurpose :Generate ;
                                                       :hasTarget :mutation_testing ;
                                                       :hasType :Deep_learning ;
                                                       :isAboutResearchTopic :CSO:Testing_and_Debugging ;
                                                       rdfs:comment """@inproceedings{caglar_development_2023,
 address = {Sivas, Turkiye},
 author = {Caglar, Osman and Taskin, Furkan and Baglum, Cem and Asik, Sergen and Yayan, Ugur},
 booktitle = {2023 {Innovations} in {Intelligent} {Systems} and {Applications} {Conference} ({ASYU})},
 copyright = {http://doi.org/10.15223/policy-029},
 doi = {10.1109/ASYU58738.2023.10296551},
 isbn = {979-8-3503-0659-0},
 month = {October},
 pages = {1--6},
 publisher = {IEEE},
 title = {Development of {Cloud} and {Artificial} {Intelligence} based {Software} {Testing} {Platform} ({ChArIoT})},
 url = {http://ieeexplore.ieee.org/document/10296551/},
 urldate = {2025-06-12},
 year = {2023}
}
""" ;
                                                       rdfs:label "caglar_development_2023" ;
                                                       rdfs:seeAlso <http://ieeexplore.ieee.org/document/10296551/> .


###  http://purl.org/ai4st/papers#calvano_leveraging_2025
<http://purl.org/ai4st/papers#calvano_leveraging_2025> rdf:type owl:NamedIndividual ,
                                                                :ResearchPaper ;
                                                       :hasLevel :AI-assisted_options ;
                                                       :hasPurpose :Generate ;
                                                       :hasTarget <http://purl.org/stc/terms#usability_testing> ;
                                                       :hasType :Generative_AI ;
                                                       :isAboutResearchTopic :CSO:Testing_and_Debugging ;
                                                       rdfs:comment """@inproceedings{calvano_leveraging_2025,
 address = {Cagliari Italy},
 author = {Calvano, Miriana and Curci, Antonio and Lanzilotti, Rosa and Piccinno, Antonio and Ragone, Azzurra},
 booktitle = {Companion {Proceedings} of the 30th {International} {Conference} on {Intelligent} {User} {Interfaces}},
 doi = {10.1145/3708557.3716341},
 isbn = {979-8-4007-1409-2},
 language = {en},
 month = {March},
 pages = {78--81},
 publisher = {ACM},
 shorttitle = {Leveraging {Large} {Language} {Models} for {Usability} {Testing}},
 title = {Leveraging {Large} {Language} {Models} for {Usability} {Testing}: a {Preliminary} {Study}},
 url = {http://dl.acm.org/doi/10.1145/3708557.3716341},
 urldate = {2025-06-12},
 year = {2025}
}
""" ;
                                                       rdfs:label "calvano_leveraging_2025" ;
                                                       rdfs:seeAlso <http://dl.acm.org/doi/10.1145/3708557.3716341> .


###  http://purl.org/ai4st/papers#confido_reinforcing_2022
<http://purl.org/ai4st/papers#confido_reinforcing_2022> rdf:type owl:NamedIndividual ,
                                                                 :ResearchPaper ;
                                                        :hasLevel :AI-driven_full_automation ;
                                                        :hasPurpose :Improve ;
                                                        :hasTarget :penetration_testing ;
                                                        :hasType :Deep_learning ;
                                                        :isAboutResearchTopic :CSO:Testing_and_Debugging ;
                                                        rdfs:comment """@inproceedings{confido_reinforcing_2022,
 address = {Big Sky, MT, USA},
 author = {Confido, Alessandro and Ntagiou, Evridiki V. and Wallum, Marcus},
 booktitle = {2022 {IEEE} {Aerospace} {Conference} ({AERO})},
 copyright = {http://doi.org/10.15223/policy-029},
 doi = {10.1109/AERO53065.2022.9843459},
 isbn = {978-1-6654-3760-8},
 month = {March},
 pages = {1--15},
 publisher = {IEEE},
 title = {Reinforcing {Penetration} {Testing} {Using} {AI}},
 url = {http://ieeexplore.ieee.org/document/9843459/},
 urldate = {2025-06-12},
 year = {2022}
}
""" ;
                                                        rdfs:label "confido_reinforcing_2022" ;
                                                        rdfs:seeAlso <http://ieeexplore.ieee.org/document/9843459/> .


###  http://purl.org/ai4st/papers#de_almeida_ai_2024
<http://purl.org/ai4st/papers#de_almeida_ai_2024> rdf:type owl:NamedIndividual ,
                                                           :ResearchPaper ;
                                                  :hasLevel :AI-assisted_options ;
                                                  :hasPurpose :Generate ;
                                                  :hasTarget <http://purl.org/stc/terms#exploratory_testing> ;
                                                  :hasType :Generative_AI ;
                                                  :isAboutResearchTopic :CSO:Testing_and_Debugging ;
                                                  rdfs:comment """@inproceedings{de_almeida_ai_2024,
 address = {Salvador Bahia Brazil},
 author = {De Almeida, Ágatha and Collins, Eliane and Oran, Ana Carolina},
 booktitle = {Proceedings of the {XXIII} {Brazilian} {Symposium} on {Software} {Quality}},
 doi = {10.1145/3701625.3701657},
 isbn = {979-8-4007-1777-2},
 language = {en},
 month = {November},
 pages = {179--188},
 publisher = {ACM},
 shorttitle = {{AI} in {Service} of {Software} {Quality}},
 title = {{AI} in {Service} of {Software} {Quality}: {How} {ChatGPT} and {Personas} {Are} {Transforming} {Exploratory} {Testing}},
 url = {http://dl.acm.org/doi/10.1145/3701625.3701657},
 urldate = {2025-06-12},
 year = {2024}
}
""" ;
                                                  rdfs:label "de_almeida_ai_2024" ;
                                                  rdfs:seeAlso <http://dl.acm.org/doi/10.1145/3701625.3701657> .


###  http://purl.org/ai4st/papers#de_santiago_junior_method_2022
<http://purl.org/ai4st/papers#de_santiago_junior_method_2022> rdf:type owl:NamedIndividual ,
                                                                       :ResearchPaper ;
                                                              :hasLevel :AI-assisted_options ;
                                                              :hasPurpose :Generate ;
                                                              :hasTarget <http://purl.org/stc/terms#test_oracle> ;
                                                              :hasType :Deep_learning ;
                                                              :isAboutResearchTopic :CSO:Testing_and_Debugging ;
                                                              rdfs:comment """@inproceedings{de_santiago_junior_method_2022,
 address = {Pittsburgh Pennsylvania},
 author = {De Santiago Júnior, Valdivino Alexandre},
 booktitle = {Proceedings of the 3rd {ACM}/{IEEE} {International} {Conference} on {Automation} of {Software} {Test}},
 doi = {10.1145/3524481.3527232},
 isbn = {978-1-4503-9286-0},
 language = {en},
 month = {May},
 pages = {40--51},
 publisher = {ACM},
 title = {A method and experiment to evaluate deep neural networks as test oracles for scientific software},
 url = {http://dl.acm.org/doi/10.1145/3524481.3527232},
 urldate = {2025-06-12},
 year = {2022}
}
""" ;
                                                              rdfs:label "de_santiago_junior_method_2022" ;
                                                              rdfs:seeAlso <http://dl.acm.org/doi/10.1145/3524481.3527232> .


###  http://purl.org/ai4st/papers#djajadi_using_nodate
<http://purl.org/ai4st/papers#djajadi_using_nodate> rdf:type owl:NamedIndividual ,
                                                             :ResearchPaper ;
                                                    :hasLevel :AI-assisted_options ;
                                                    :hasPurpose :Generate ,
                                                                :Understand ;
                                                    :hasTarget :test_documentation ;
                                                    :hasType :Generative_AI ;
                                                    :isAboutResearchTopic :CSO:Testing_and_Debugging ;
                                                    rdfs:comment """@inproceedings{djajadi_using_nodate,
 author = {Djajadi, Natanael and Deljouyi, Amirhossein and Zaidman, Andy},
 booktitle = {Early {Research} {Achievements} ({ERA})},
 doi = {10.1109/ICPC66645.2025.00040},
 title = {Using {Large} {Language} {Models} to {Generate} {Concise} and {Understandable} {Test} {Case} {Summaries}},
 url = {http://azaidman.github.io/publications/djajadiICPC2025.pdf},
 urldate = {2025-06-12}
}""" ;
                                                    rdfs:label "djajadi_using_nodate" ;
                                                    rdfs:seeAlso <http://azaidman.github.io/publications/djajadiICPC2025.pdf> .


###  http://purl.org/ai4st/papers#ferreira_acceptance_2025
<http://purl.org/ai4st/papers#ferreira_acceptance_2025> rdf:type owl:NamedIndividual ,
                                                                 :ResearchPaper ;
                                                        :hasLevel :AI-assisted_selection ;
                                                        :hasPurpose :Generate ;
                                                        :hasTarget :Web_application ,
                                                                   <http://purl.org/stc/terms#acceptance_testing> ,
                                                                   <http://purl.org/stc/terms#test_automation> ;
                                                        :hasType :Generative_AI ;
                                                        :isAboutResearchTopic :CSO:Testing_and_Debugging ;
                                                        rdfs:comment """@misc{ferreira_acceptance_2025,
 author = {Ferreira, Margarida and Viegas, Luis and Faria, Joao Pascoal and Lima, Bruno},
 doi = {10.48550/arXiv.2504.07244},
 keywords = {Computer Science - Software Engineering},
 month = {April},
 note = {arXiv:2504.07244 [cs]},
 publisher = {arXiv},
 shorttitle = {Acceptance {Test} {Generation} with {Large} {Language} {Models}},
 title = {Acceptance {Test} {Generation} with {Large} {Language} {Models}: {An} {Industrial} {Case} {Study}},
 url = {http://arxiv.org/abs/2504.07244},
 urldate = {2025-06-12},
 year = {2025}
}""" ;
                                                        rdfs:label "ferreira_acceptance_2025" ;
                                                        rdfs:seeAlso <http://arxiv.org/abs/2504.07244> .


###  http://purl.org/ai4st/papers#franzosi_llm-based_2025
<http://purl.org/ai4st/papers#franzosi_llm-based_2025> rdf:type owl:NamedIndividual ,
                                                                :ResearchPaper ;
                                                       :hasLevel :AI-driven_partial_automation ;
                                                       :hasPurpose :Generate ;
                                                       :hasTarget <http://purl.org/stc/terms#GUI_testing> ,
                                                                  <http://purl.org/stc/terms#test_report> ;
                                                       :hasType :Generative_AI ;
                                                       :isAboutResearchTopic :CSO:Testing_and_Debugging ;
                                                       rdfs:comment """@inproceedings{franzosi_llm-based_2025,
 address = {Napoli, Italy},
 author = {Franzosi, Diogo Buarque and Alégroth, Emil and Isaac, Maycel},
 booktitle = {2025 {IEEE} {Conference} on {Software} {Testing}, {Verification} and {Validation} ({ICST})},
 copyright = {http://doi.org/10.15223/policy-029},
 doi = {10.1109/ICST62969.2025.10988984},
 isbn = {979-8-3315-0814-2},
 month = {March},
 pages = {453--463},
 publisher = {IEEE},
 title = {{LLM}-{Based} {Labelling} of {Recorded} {Automated} {GUI}-{Based} {Test} {Cases}},
 url = {http://ieeexplore.ieee.org/document/10988984/},
 urldate = {2025-06-12},
 year = {2025}
}
""" ;
                                                       rdfs:label "franzosi_llm-based_2025" ;
                                                       rdfs:seeAlso <http://ieeexplore.ieee.org/document/10988984/> .


###  http://purl.org/ai4st/papers#gamal_owl_2023
<http://purl.org/ai4st/papers#gamal_owl_2023> rdf:type owl:NamedIndividual ,
                                                       :ResearchPaper ;
                                              :hasLevel :AI-driven_full_automation ;
                                              :hasPurpose :Generate ;
                                              :hasTarget <http://purl.org/ai4st/new_terms#visual_testing> ,
                                                         <http://purl.org/stc/terms#GUI_testing> ;
                                              :hasType :Deep_learning ;
                                              :isAboutResearchTopic :CSO:Testing_and_Debugging ;
                                              rdfs:comment """@inproceedings{gamal_owl_2023,
 address = {Giza, Egypt},
 author = {Gamal, Ahmed and Emad, Reem and Mohamed, Taher and Mohamed, Omar and Hamdy, Ahmed and Ali, Sarah},
 booktitle = {2023 5th {Novel} {Intelligent} and {Leading} {Emerging} {Sciences} {Conference} ({NILES})},
 copyright = {http://doi.org/10.15223/policy-029},
 doi = {10.1109/NILES59815.2023.10296575},
 isbn = {979-8-3503-8103-0},
 month = {October},
 pages = {312--315},
 publisher = {IEEE},
 shorttitle = {Owl {Eye}},
 title = {Owl {Eye}: {An} {AI}-{Driven} {Visual} {Testing} {Tool}},
 url = {http://ieeexplore.ieee.org/document/10296575/},
 urldate = {2025-06-12},
 year = {2023}
}
""" ;
                                              rdfs:label "gamal_owl_2023" ;
                                              rdfs:seeAlso <http://ieeexplore.ieee.org/document/10296575/> .


###  http://purl.org/ai4st/papers#gao_approach_2022
<http://purl.org/ai4st/papers#gao_approach_2022> rdf:type owl:NamedIndividual ,
                                                          :ResearchPaper ;
                                                 :hasLevel :AI-assisted_selection ;
                                                 :hasPurpose :Generate ;
                                                 :hasTarget <http://purl.org/stc/terms#GUI_testing> ;
                                                 :hasType :Deep_learning ;
                                                 :isAboutResearchTopic :CSO:Testing_and_Debugging ;
                                                 rdfs:comment """@inproceedings{gao_approach_2022,
 address = {Newark, CA, USA},
 author = {Gao, Jerry and Li, ShiTing and Tao, Chuanqi and He, Yejun and Anumalasetty, Amrutha Pavani and Joseph, Erica Wilson and Sripathi, Akshata Hatwar Kumbashi and Nayani, Himabindu},
 booktitle = {2022 {IEEE} {International} {Conference} {On} {Artificial} {Intelligence} {Testing} ({AITest})},
 copyright = {http://doi.org/10.15223/policy-029},
 doi = {10.1109/AITest55621.2022.00020},
 isbn = {978-1-6654-8737-5},
 month = {August},
 pages = {79--86},
 publisher = {IEEE},
 title = {An {Approach} to {GUI} {Test} {Scenario} {Generation} {Using} {Machine} {Learning}},
 url = {http://ieeexplore.ieee.org/document/9898132/},
 urldate = {2025-06-12},
 year = {2022}
}
""" ;
                                                 rdfs:label "gao_approach_2022" ;
                                                 rdfs:seeAlso <http://ieeexplore.ieee.org/document/9898132/> .


###  http://purl.org/ai4st/papers#gao_clozemaster_2025
<http://purl.org/ai4st/papers#gao_clozemaster_2025> rdf:type owl:NamedIndividual ,
                                                             :ResearchPaper ;
                                                    :hasLevel :AI-driven_full_automation ;
                                                    :hasPurpose :Generate ;
                                                    :hasTarget :test_generation ;
                                                    :hasType :Generative_AI ;
                                                    :isAboutResearchTopic :CSO:Testing_and_Debugging ;
                                                    rdfs:comment """@inproceedings{gao_clozemaster_2025,
 author = {Gao, Hongyan and Yang, Yibiao and Sun, Maolin and Wu, Jiangchang and Zhou, Yuming and Xu, Baowen},
 doi = {10.1109/ICSE55347.2025.00175},
 isbn = {979-8-3315-0569-1},
 language = {English},
 month = {March},
 note = {ISSN: 1558-1225},
 pages = {712--712},
 publisher = {IEEE Computer Society},
 shorttitle = {{ClozeMaster}},
 title = {{ClozeMaster}: {Fuzzing} {Rust} {Compiler} by {Harnessing} {LLMs} for {Infilling} {Masked} {Real} {Programs}},
 url = {http://www.computer.org/csdl/proceedings-article/icse/2025/056900a712/251mH1NLq1y},
 urldate = {2025-06-12},
 year = {2025}
}
""" ;
                                                    rdfs:label "gao_clozemaster_2025" ;
                                                    rdfs:seeAlso <http://www.computer.org/csdl/proceedings-article/icse/2025/056900a712/251mH1NLq1y> .


###  http://purl.org/ai4st/papers#garg_generative_2023
<http://purl.org/ai4st/papers#garg_generative_2023> rdf:type owl:NamedIndividual ,
                                                             :ResearchPaper ;
                                                    :hasLevel :AI-assisted_selection ;
                                                    :hasPurpose :Generate ;
                                                    :hasTarget :ERP_system ,
                                                               :test_generation ;
                                                    :hasType :Generative_AI ;
                                                    :isAboutResearchTopic :CSO:Testing_and_Debugging ;
                                                    rdfs:comment """@inproceedings{garg_generative_2023,
 address = {Faridabad, India},
 author = {Garg, Anshumaan and Sharma, Dolly},
 booktitle = {2023 {International} {Conference} on {Advances} in {Computation}, {Communication} and {Information} {Technology} ({ICAICCIT})},
 copyright = {http://doi.org/10.15223/policy-029},
 doi = {10.1109/ICAICCIT60255.2023.10466102},
 isbn = {979-8-3503-4438-7},
 month = {November},
 pages = {187--193},
 publisher = {IEEE},
 title = {Generative {AI} for {Software} {Test} {Modelling} with a focus on {ERP} {Software}},
 url = {http://ieeexplore.ieee.org/document/10466102/},
 urldate = {2025-06-12},
 year = {2023}
}
""" ;
                                                    rdfs:label "garg_generative_2023" ;
                                                    rdfs:seeAlso <http://ieeexplore.ieee.org/document/10466102/> .


###  http://purl.org/ai4st/papers#garlapati_ai-powered_2024
<http://purl.org/ai4st/papers#garlapati_ai-powered_2024> rdf:type owl:NamedIndividual ,
                                                                  :ResearchPaper ;
                                                         :hasLevel :AI-driven_partial_automation ;
                                                         :hasPurpose :Generate ;
                                                         :hasTarget <http://purl.org/stc/terms#component_testing> ;
                                                         :hasType :Generative_AI ;
                                                         :isAboutResearchTopic :CSO:Testing_and_Debugging ;
                                                         rdfs:comment """@inproceedings{garlapati_ai-powered_2024,
 address = {Bangalore, India},
 author = {Garlapati, Anusha and Satya Sai Muni Parmesh, M N V and {Savitha} and S, Jaisri},
 booktitle = {2024 5th {IEEE} {Global} {Conference} for {Advancement} in {Technology} ({GCAT})},
 copyright = {http://doi.org/10.15223/policy-029},
 doi = {10.1109/GCAT62922.2024.10923987},
 isbn = {979-8-3503-7666-1 979-8-3503-7668-5},
 month = {October},
 pages = {1--5},
 publisher = {IEEE},
 shorttitle = {{AI}-{Powered} {Multi}-{Agent} {Framework} for {Automated} {Unit} {Test} {Case} {Generation}},
 title = {{AI}-{Powered} {Multi}-{Agent} {Framework} for {Automated} {Unit} {Test} {Case} {Generation}: {Enhancing} {Software} {Quality} through {LLM}’s},
 url = {http://ieeexplore.ieee.org/document/10923987/},
 urldate = {2025-06-12},
 year = {2024}
}
""" ;
                                                         rdfs:label "garlapati_ai-powered_2024" ;
                                                         rdfs:seeAlso <http://ieeexplore.ieee.org/document/10923987/> .


###  http://purl.org/ai4st/papers#ghimis_river_2020
<http://purl.org/ai4st/papers#ghimis_river_2020> rdf:type owl:NamedIndividual ,
                                                          :ResearchPaper ;
                                                 :hasLevel :AI-driven_full_automation ;
                                                 :hasPurpose :Improve ;
                                                 :hasTarget :concolic_testing ,
                                                            <http://purl.org/stc/terms#security_testing> ,
                                                            <http://purl.org/stc/terms#test_automation> ;
                                                 :hasType :Deep_learning ;
                                                 :isAboutResearchTopic :CSO:Testing_and_Debugging ;
                                                 rdfs:comment """@inproceedings{ghimis_river_2020,
 address = {Virtual USA},
 author = {Ghimis, Bogdan and Paduraru, Miruna and Stefanescu, Alin},
 booktitle = {Proceedings of the 1st {ACM} {SIGSOFT} {International} {Workshop} on {Languages} and {Tools} for {Next}-{Generation} {Testing}},
 doi = {10.1145/3416504.3424335},
 isbn = {978-1-4503-8123-9},
 language = {en},
 month = {November},
 pages = {13--18},
 publisher = {ACM},
 shorttitle = {{RIVER} 2.0},
 title = {{RIVER} 2.0: an open-source testing framework using {AI} techniques},
 url = {http://dl.acm.org/doi/10.1145/3416504.3424335},
 urldate = {2025-06-12},
 year = {2020}
}
""" ;
                                                 rdfs:label "ghimis_river_2020" ;
                                                 rdfs:seeAlso <http://dl.acm.org/doi/10.1145/3416504.3424335> .


###  http://purl.org/ai4st/papers#hagar_ais_2025
<http://purl.org/ai4st/papers#hagar_ais_2025> rdf:type owl:NamedIndividual ,
                                                       :ResearchPaper ;
                                              :hasLevel :No_AI_automation ;
                                              :hasPurpose :Understand ;
                                              :hasTarget <http://purl.org/stc/terms#test_approach> ;
                                              :hasType :Generative_AI ;
                                              :isAboutResearchTopic :CSO:Testing_and_Debugging ;
                                              rdfs:comment """@inproceedings{hagar_ais_2025,
 address = {Naples, Italy},
 author = {Hagar, Jon and Wissink, Tome},
 booktitle = {2025 {IEEE} {International} {Conference} on {Software} {Testing}, {Verification} and {Validation} {Workshops} ({ICSTW})},
 copyright = {http://doi.org/10.15223/policy-029},
 doi = {10.1109/ICSTW64639.2025.10962517},
 isbn = {979-8-3315-3467-7},
 month = {March},
 pages = {194--199},
 publisher = {IEEE},
 title = {{AIs} {Understanding} of {Software} {Test} {Architecture}},
 url = {http://ieeexplore.ieee.org/document/10962517/},
 urldate = {2025-06-12},
 year = {2025}
}
""" ;
                                              rdfs:label "hagar_ais_2025" ;
                                              rdfs:seeAlso <http://ieeexplore.ieee.org/document/10962517/> .


###  http://purl.org/ai4st/papers#haldar_wip_2024
<http://purl.org/ai4st/papers#haldar_wip_2024> rdf:type owl:NamedIndividual ,
                                                        :ResearchPaper ;
                                               :hasLevel :No_AI_automation ;
                                               :hasPurpose :Understand ;
                                               :hasTarget <http://purl.org/stc/terms#testing> ;
                                               :hasType :Generative_AI ;
                                               :isAboutResearchTopic :CSO:Testing_and_Debugging ;
                                               rdfs:comment """@inproceedings{haldar_wip_2024,
 address = {Washington, DC, USA},
 author = {Haldar, Susmita and Pierce, Mary and Capretz, Luiz Fernando},
 booktitle = {2024 {IEEE} {Frontiers} in {Education} {Conference} ({FIE})},
 copyright = {http://doi.org/10.15223/policy-029},
 doi = {10.1109/FIE61694.2024.10893214},
 isbn = {979-8-3503-5150-7},
 month = {October},
 pages = {1--5},
 publisher = {IEEE},
 shorttitle = {{WIP}},
 title = {{WIP}: {Assessing} the {Effectiveness} of {ChatGPT} in {Preparatory} {Testing} {Activities}},
 url = {http://ieeexplore.ieee.org/document/10893214/},
 urldate = {2025-06-12},
 year = {2024}
}
""" ;
                                               rdfs:label "haldar_wip_2024" ;
                                               rdfs:seeAlso <http://ieeexplore.ieee.org/document/10893214/> .


###  http://purl.org/ai4st/papers#happe_getting_2023
<http://purl.org/ai4st/papers#happe_getting_2023> rdf:type owl:NamedIndividual ,
                                                           :ResearchPaper ;
                                                  :hasLevel :AI-assisted_selection ;
                                                  :hasPurpose :Generate ,
                                                              :Understand ;
                                                  :hasTarget :penetration_testing ;
                                                  :hasType :Generative_AI ;
                                                  :isAboutResearchTopic :CSO:Testing_and_Debugging ;
                                                  rdfs:comment """@inproceedings{happe_getting_2023,
 address = {San Francisco CA USA},
 author = {Happe, Andreas and Cito, Jürgen},
 booktitle = {Proceedings of the 31st {ACM} {Joint} {European} {Software} {Engineering} {Conference} and {Symposium} on the {Foundations} of {Software} {Engineering}},
 doi = {10.1145/3611643.3613083},
 isbn = {979-8-4007-0327-0},
 language = {en},
 month = {November},
 pages = {2082--2086},
 publisher = {ACM},
 shorttitle = {Getting pwn’d by {AI}},
 title = {Getting pwn’d by {AI}: {Penetration} {Testing} with {Large} {Language} {Models}},
 url = {http://dl.acm.org/doi/10.1145/3611643.3613083},
 urldate = {2025-06-12},
 year = {2023}
}""" ;
                                                  rdfs:label "happe_getting_2023" ;
                                                  rdfs:seeAlso <http://dl.acm.org/doi/10.1145/3611643.3613083> .


###  http://purl.org/ai4st/papers#helmy_ai-driven_2024
<http://purl.org/ai4st/papers#helmy_ai-driven_2024> rdf:type owl:NamedIndividual ,
                                                             :ResearchPaper ;
                                                    :hasLevel :AI-assisted_selection ;
                                                    :hasPurpose :Generate ;
                                                    :hasTarget <http://purl.org/stc/terms#component_testing> ;
                                                    :hasType :Generative_AI ;
                                                    :isAboutResearchTopic :CSO:Testing_and_Debugging ;
                                                    rdfs:comment """@inproceedings{helmy_ai-driven_2024,
 address = {Cairo, Egypt},
 author = {Helmy, Mona and Sobhy, Omar and ElHusseiny, Farida},
 booktitle = {2024 {International} {Telecommunications} {Conference} ({ITC}-{Egypt})},
 copyright = {http://doi.org/10.15223/policy-029},
 doi = {10.1109/ITC-Egypt61547.2024.10620598},
 isbn = {979-8-3503-5140-8},
 month = {July},
 pages = {1--6},
 publisher = {IEEE},
 shorttitle = {{AI}-{Driven} {Testing}},
 title = {{AI}-{Driven} {Testing}: {Unleashing} {Autonomous} {Systems} for {Superior} {Software} {Quality} {Using} {Generative} {AI}},
 url = {http://ieeexplore.ieee.org/document/10620598/},
 urldate = {2025-06-12},
 year = {2024}
}
""" ;
                                                    rdfs:label "helmy_ai-driven_2024" ;
                                                    rdfs:seeAlso <http://ieeexplore.ieee.org/document/10620598/> .


###  http://purl.org/ai4st/papers#hossain_togll_2024
<http://purl.org/ai4st/papers#hossain_togll_2024> rdf:type owl:NamedIndividual ,
                                                           :ResearchPaper ;
                                                  :hasLevel :AI-driven_partial_automation ;
                                                  :hasPurpose :Generate ;
                                                  :hasTarget <http://purl.org/stc/terms#test_oracle> ;
                                                  :hasType :Generative_AI ;
                                                  :isAboutResearchTopic :CSO:Testing_and_Debugging ;
                                                  rdfs:comment """@misc{hossain_togll_2024,
 author = {Hossain, Soneya Binta and Dwyer, Matthew},
 doi = {10.48550/arXiv.2405.03786},
 keywords = {Computer Science - Software Engineering},
 month = {December},
 note = {arXiv:2405.03786 [cs]},
 publisher = {arXiv},
 shorttitle = {{TOGLL}},
 title = {{TOGLL}: {Correct} and {Strong} {Test} {Oracle} {Generation} with {LLMs}},
 url = {http://arxiv.org/abs/2405.03786},
 urldate = {2025-06-13},
 year = {2024}
}""" ;
                                                  rdfs:label "hossain_togll_2024" ;
                                                  rdfs:seeAlso <http://arxiv.org/abs/2405.03786> .


###  http://purl.org/ai4st/papers#kapoor_ai-assisted_2025
<http://purl.org/ai4st/papers#kapoor_ai-assisted_2025> rdf:type owl:NamedIndividual ,
                                                                :ResearchPaper ;
                                                       :hasLevel :AI-assisted_options ;
                                                       :hasPurpose :Generate ;
                                                       :hasTarget <http://purl.org/stc/terms#GUI_testing> ;
                                                       :hasType :Deep_learning ;
                                                       :isAboutResearchTopic :CSO:Testing_and_Debugging ;
                                                       rdfs:comment """@inproceedings{kapoor_ai-assisted_2025,
 address = {Bhilai, India},
 author = {Kapoor, Saurabh},
 booktitle = {2025 {Fifth} {International} {Conference} on {Advances} in {Electrical}, {Computing}, {Communication} and {Sustainable} {Technologies} ({ICAECT})},
 copyright = {http://doi.org/10.15223/policy-029},
 doi = {10.1109/ICAECT63952.2025.10958949},
 isbn = {979-8-3503-5623-6},
 month = {January},
 pages = {1--5},
 publisher = {IEEE},
 title = {{AI}-{Assisted} {Test} {Script} {Generation} for {GUI} {Applications}},
 url = {http://ieeexplore.ieee.org/document/10958949/},
 urldate = {2025-06-12},
 year = {2025}
}
""" ;
                                                       rdfs:label "kapoor_ai-assisted_2025" ;
                                                       rdfs:seeAlso <http://ieeexplore.ieee.org/document/10958949/> .


###  http://purl.org/ai4st/papers#kaur_approach_2020
<http://purl.org/ai4st/papers#kaur_approach_2020> rdf:type owl:NamedIndividual ,
                                                           :ResearchPaper ;
                                                  :hasLevel :AI-assisted_options ;
                                                  :hasPurpose :Improve ;
                                                  :hasTarget <http://purl.org/stc/terms#regression_testing> ;
                                                  :hasType :Swarm_intelligence ;
                                                  :isAboutResearchTopic :CSO:Testing_and_Debugging ;
                                                  rdfs:comment """@inproceedings{kaur_approach_2020,
 address = {Noida, India},
 author = {Kaur, Amandeep},
 booktitle = {2020 10th {International} {Conference} on {Cloud} {Computing}, {Data} {Science} \\& {Engineering} ({Confluence})},
 copyright = {http://ieeexplore.ieee.org/Xplorehelp/downloads/license-information/IEEE.html},
 doi = {10.1109/Confluence47617.2020.9058244},
 isbn = {978-1-7281-2791-0},
 month = {January},
 pages = {649--654},
 publisher = {IEEE},
 title = {An {Approach} {To} {Extract} {Optimal} {Test} {Cases} {Using} {AI}},
 url = {http://ieeexplore.ieee.org/document/9058244/},
 urldate = {2025-06-12},
 year = {2020}
}
""" ;
                                                  rdfs:label "kaur_approach_2020" ;
                                                  rdfs:seeAlso <http://ieeexplore.ieee.org/document/9058244/> .


###  http://purl.org/ai4st/papers#leu_reducing_2024
<http://purl.org/ai4st/papers#leu_reducing_2024> rdf:type owl:NamedIndividual ,
                                                          :ResearchPaper ;
                                                 :hasLevel :AI-assisted_options ;
                                                 :hasPurpose :Generate ;
                                                 :hasTarget <http://purl.org/stc/terms#API_testing> ,
                                                            <http://purl.org/stc/terms#test_automation> ;
                                                 :hasType :Deep_learning ;
                                                 :isAboutResearchTopic :CSO:Testing_and_Debugging ;
                                                 rdfs:comment ""@inproceedings{leu_reducing_2024,  address = {lisbon portugal},  author = {leu, benjamin and volken, jonas and kropp, martin and dogru, nejdet and anslow, craig and biddle, robert},  booktitle = {proceedings of the 5th {acm}/{ieee} {international} {conference} on {automation} of {software} {test} ({ast} 2024)},  doi = {10.1145/3644032.3644449},  isbn = {979-8-4007-0588-5},  language = {en},  month = {april},  pages = {147--148},  publisher = {acm},  title = {reducing {workload} in {using} {ai}-based {api} {rest} {test} {generation}},  url = {http://dl.acm.org/doi/10.1145/3644032.3644449},  urldate = {2025-06-12},  year = {2024} } ;
                                                 rdfs:label "leu_reducing_2024" ;
                                                 rdfs:seeAlso <http://dl.acm.org/doi/10.1145/3644032.3644449> .


###  http://purl.org/ai4st/papers#maia_ai-driven_2024
<http://purl.org/ai4st/papers#maia_ai-driven_2024> rdf:type owl:NamedIndividual ,
                                                            :ResearchPaper ;
                                                   :hasLevel :No_AI_automation ;
                                                   :hasPurpose :Understand ;
                                                   :hasTarget <http://purl.org/stc/terms#acceptance_testing> ;
                                                   :hasType :Generative_AI ;
                                                   :isAboutResearchTopic :CSO:Testing_and_Debugging ;
                                                   rdfs:comment """@inproceedings{maia_ai-driven_2024,
 address = {Salvador Bahia Brazil},
 author = {Maia, Caio Jordan De Lima and Aguiar, Yuska Paola Costa},
 booktitle = {Proceedings of the {XXIII} {Brazilian} {Symposium} on {Software} {Quality}},
 doi = {10.1145/3701625.3701691},
 isbn = {979-8-4007-1777-2},
 language = {en},
 month = {November},
 pages = {665--672},
 publisher = {ACM},
 shorttitle = {{AI}-{Driven} {Acceptance} {Testing}},
 title = {{AI}-{Driven} {Acceptance} {Testing}: first insights exploring the educational potential for test analysts},
 url = {http://dl.acm.org/doi/10.1145/3701625.3701691},
 urldate = {2025-06-12},
 year = {2024}
}
""" ;
                                                   rdfs:label "maia_ai-driven_2024" ;
                                                   rdfs:seeAlso <http://dl.acm.org/doi/10.1145/3701625.3701691> .


###  http://purl.org/ai4st/papers#martin-lopez_ai-driven_2020
<http://purl.org/ai4st/papers#martin-lopez_ai-driven_2020> rdf:type owl:NamedIndividual ,
                                                                    :ResearchPaper ;
                                                           :hasLevel :AI-driven_full_automation ;
                                                           :hasPurpose :Generate ;
                                                           :hasTarget <http://purl.org/stc/terms#API_testing> ;
                                                           :hasType :Classical_machine_learning ;
                                                           :isAboutResearchTopic :CSO:Testing_and_Debugging ;
                                                           rdfs:comment """@inproceedings{martin-lopez_ai-driven_2020,
 address = {Seoul South Korea},
 author = {Martin-Lopez, Alberto},
 booktitle = {Proceedings of the {ACM}/{IEEE} 42nd {International} {Conference} on {Software} {Engineering}: {Companion} {Proceedings}},
 doi = {10.1145/3377812.3381388},
 isbn = {978-1-4503-7122-3},
 language = {en},
 month = {June},
 pages = {202--205},
 publisher = {ACM},
 title = {{AI}-driven web {API} testing},
 url = {http://dl.acm.org/doi/10.1145/3377812.3381388},
 urldate = {2025-06-12},
 year = {2020}
}
""" ;
                                                           rdfs:label "martin-lopez_ai-driven_2020" ;
                                                           rdfs:seeAlso <http://dl.acm.org/doi/10.1145/3377812.3381388> .


###  http://purl.org/ai4st/papers#mohacsi_ai-based_2021
<http://purl.org/ai4st/papers#mohacsi_ai-based_2021> rdf:type owl:NamedIndividual ,
                                                              :ResearchPaper ;
                                                     :hasLevel :AI-assisted_options ;
                                                     :hasPurpose :Improve ;
                                                     :hasTarget <http://purl.org/stc/terms#test_model> ;
                                                     :hasType :Classical_machine_learning ;
                                                     :isAboutResearchTopic :CSO:Testing_and_Debugging ;
                                                     rdfs:comment """@inproceedings{mohacsi_ai-based_2021,
 address = {Honolulu, HI, USA},
 author = {Mohacsi, Stefan and Felderer, Michael},
 booktitle = {2021 {IEEE} {International} {Conference} on {Software} {Analysis}, {Evolution} and {Reengineering} ({SANER})},
 copyright = {http://ieeexplore.ieee.org/Xplorehelp/downloads/license-information/IEEE.html},
 doi = {10.1109/SANER50967.2021.00080},
 isbn = {978-1-7281-9630-5},
 month = {March},
 pages = {636--638},
 publisher = {IEEE},
 title = {{AI}-{Based} {Enhancement} of {Test} {Models} in an {Industrial} {Model}-{Based} {Testing} {Tool}},
 url = {http://ieeexplore.ieee.org/document/9426031/},
 urldate = {2025-06-12},
 year = {2021}
}
""" ;
                                                     rdfs:label "mohacsi_ai-based_2021" ;
                                                     rdfs:seeAlso <http://ieeexplore.ieee.org/document/9426031/> .


###  http://purl.org/ai4st/papers#naimi_new_2024
<http://purl.org/ai4st/papers#naimi_new_2024> rdf:type owl:NamedIndividual ,
                                                       :ResearchPaper ;
                                              :hasLevel :AI-assisted_options ;
                                              :hasPurpose :Generate ;
                                              :hasTarget <http://purl.org/stc/terms#model_based_testing> ;
                                              :hasType :Generative_AI ;
                                              :isAboutResearchTopic :CSO:Testing_and_Debugging ;
                                              rdfs:comment """@inproceedings{naimi_new_2024,
 address = {Fes, Morocco},
 author = {Naimi, Lahbib and Bouziane, El Mahi and Manaouch, Mohamed and Jakimi, Abdeslam},
 booktitle = {2024 {International} {Conference} on {Circuit}, {Systems} and {Communication} ({ICCSC})},
 copyright = {http://doi.org/10.15223/policy-029},
 doi = {10.1109/ICCSC62074.2024.10616548},
 isbn = {979-8-3503-6530-6},
 month = {June},
 pages = {1--5},
 publisher = {IEEE},
 title = {A new approach for automatic test case generation from use case diagram using {LLMs} and prompt engineering},
 url = {http://ieeexplore.ieee.org/document/10616548/},
 urldate = {2025-06-12},
 year = {2024}
}
""" ;
                                              rdfs:label "naimi_new_2024" ;
                                              rdfs:seeAlso <http://ieeexplore.ieee.org/document/10616548/> .


###  http://purl.org/ai4st/papers#olmez_automation_2024
<http://purl.org/ai4st/papers#olmez_automation_2024> rdf:type owl:NamedIndividual ,
                                                              :ResearchPaper ;
                                                     :hasLevel :AI-assisted_options ;
                                                     :hasPurpose :Generate ;
                                                     :hasTarget <http://purl.org/stc/terms#test_driven_development> ;
                                                     :hasType :Deep_learning ;
                                                     :isAboutResearchTopic :CSO:Testing_and_Debugging ;
                                                     rdfs:comment """@inproceedings{olmez_automation_2024,
 address = {Würzburg, Germany},
 author = {Olmez, Muhammet Mustafa and Gehringer, Edward},
 booktitle = {2024 36th {International} {Conference} on {Software} {Engineering} {Education} and {Training} ({CSEE}\\&amp;{T})},
 copyright = {http://doi.org/10.15223/policy-029},
 doi = {10.1109/CSEET62301.2024.10663016},
 isbn = {979-8-3503-7897-9},
 month = {July},
 pages = {1--10},
 publisher = {IEEE},
 title = {Automation of {Test} {Skeletons} {Within} {Test}-{Driven} {Development} {Projects}},
 url = {http://ieeexplore.ieee.org/document/10663016/},
 urldate = {2025-06-12},
 year = {2024}
}
""" ;
                                                     rdfs:label "olmez_automation_2024" ;
                                                     rdfs:seeAlso <http://ieeexplore.ieee.org/document/10663016/> .


###  http://purl.org/ai4st/papers#peixoto_effectiveness_2025
<http://purl.org/ai4st/papers#peixoto_effectiveness_2025> rdf:type owl:NamedIndividual ,
                                                                   :ResearchPaper ;
                                                          :hasLevel :AI-assisted_options ;
                                                          :hasPurpose :Improve ;
                                                          :hasTarget :test_verification ;
                                                          :hasType :Generative_AI ;
                                                          :isAboutResearchTopic :CSO:Testing_and_Debugging ;
                                                          rdfs:comment """@inproceedings{peixoto_effectiveness_2025,
 address = {Ottawa, ON, Canada},
 author = {Peixoto, Myron and Baía, Davy and Nascimento, Nathalia and Alencar, Paulo and Fonseca, Baldoino and Ribeiro, Márcio},
 booktitle = {2025 {IEEE}/{ACM} {International} {Workshop} on {Deep} {Learning} for {Testing} and {Testing} for {Deep} {Learning} ({DeepTest})},
 copyright = {http://doi.org/10.15223/policy-029},
 doi = {10.1109/DeepTest66595.2025.00012},
 isbn = {979-8-3315-0190-7},
 month = {May},
 pages = {45--52},
 publisher = {IEEE},
 title = {On the {Effectiveness} of {LLMs} for {Manual} {Test} {Verifications}},
 url = {http://ieeexplore.ieee.org/document/11026915/},
 urldate = {2025-06-12},
 year = {2025}
}
""" ;
                                                          rdfs:label "peixoto_effectiveness_2025" ;
                                                          rdfs:seeAlso <http://ieeexplore.ieee.org/document/11026915/> .


###  http://purl.org/ai4st/papers#prasetya_agent-based_2021
<http://purl.org/ai4st/papers#prasetya_agent-based_2021> rdf:type owl:NamedIndividual ,
                                                                  :ResearchPaper ;
                                                         :hasLevel :Agentic_AI ;
                                                         :hasPurpose :Generate ;
                                                         :hasTarget <http://purl.org/ai4st/new_terms#visual_testing> ;
                                                         :hasType :Agentic_AI ;
                                                         :isAboutResearchTopic :CSO:Testing_and_Debugging ;
                                                         rdfs:comment """@inproceedings{prasetya_agent-based_2021,
 address = {Porto de Galinhas, Brazil},
 author = {Prasetya, I. S. W. B. and Shirzadehhajimahmood, Samira and Ansari, Saba Gholizadeh and Fernandes, Pedro and Prada, Rui},
 booktitle = {2021 {IEEE} {International} {Conference} on {Software} {Testing}, {Verification} and {Validation} {Workshops} ({ICSTW})},
 copyright = {http://doi.org/10.15223/policy-029},
 doi = {10.1109/ICSTW52544.2021.00044},
 isbn = {978-1-6654-4456-9},
 month = {April},
 pages = {213--217},
 publisher = {IEEE},
 title = {An {Agent}-based {Architecture} for {AI}-{Enhanced} {Automated} {Testing} for {XR} {Systems}},
 url = {http://ieeexplore.ieee.org/document/9440175/},
 urldate = {2025-06-12},
 year = {2021}
}""" ;
                                                         rdfs:label "prasetya_agent-based_2021" ;
                                                         rdfs:seeAlso <http://ieeexplore.ieee.org/document/9440175/> .


###  http://purl.org/ai4st/papers#primbs_assert5_2025
<http://purl.org/ai4st/papers#primbs_assert5_2025> rdf:type owl:NamedIndividual ,
                                                            :ResearchPaper ;
                                                   :hasLevel :AI-driven_partial_automation ;
                                                   :hasPurpose :Generate ;
                                                   :hasTarget :assertion ;
                                                   :hasType :Generative_AI ;
                                                   :isAboutResearchTopic :CSO:Testing_and_Debugging ;
                                                   rdfs:comment """@misc{primbs_assert5_2025,
 author = {Primbs, Severin and Fein, Benedikt and Fraser, Gordon},
 doi = {10.1109/AST66626.2025.00008},
 keywords = {Computer Science - Software Engineering},
 month = {February},
 note = {arXiv:2502.02708 [cs]},
 shorttitle = {{AsserT5}},
 title = {{AsserT5}: {Test} {Assertion} {Generation} {Using} a {Fine}-{Tuned} {Code} {Language} {Model}},
 url = {http://arxiv.org/abs/2502.02708},
 urldate = {2025-06-12},
 year = {2025}
}""" ;
                                                   rdfs:label "primbs_assert5_2025" ;
                                                   rdfs:seeAlso <http://arxiv.org/abs/2502.02708> .


###  http://purl.org/ai4st/papers#ragel_visual_2023
<http://purl.org/ai4st/papers#ragel_visual_2023> rdf:type owl:NamedIndividual ,
                                                          :ResearchPaper ;
                                                 :hasLevel :AI-assisted_options ;
                                                 :hasPurpose :Generate ;
                                                 :hasTarget <http://purl.org/ai4st/new_terms#visual_testing> ,
                                                            <http://purl.org/stc/terms#test_automation> ;
                                                 :hasType :Deep_learning ;
                                                 :isAboutResearchTopic :CSO:Testing_and_Debugging ;
                                                 rdfs:comment """@inproceedings{ragel_visual_2023,
 address = {Coron, Palawan, Philippines},
 author = {Ragel, Ritz Kevin C. and Balahadia, Francis F.},
 booktitle = {2023 {IEEE} 15th {International} {Conference} on {Humanoid}, {Nanotechnology}, {Information} {Technology}, {Communication} and {Control}, {Environment}, and {Management} ({HNICEM})},
 copyright = {http://doi.org/10.15223/policy-029},
 doi = {10.1109/HNICEM60674.2023.10589222},
 isbn = {979-8-3503-8117-7},
 month = {November},
 pages = {1--5},
 publisher = {IEEE},
 shorttitle = {Visual {Test} {Framework}},
 title = {Visual {Test} {Framework}: {Enhancing} {Software} {Test} {Automation} with {Visual} {Artificial} {Intelligence} and {Behavioral} {Driven} {Development}},
 url = {http://ieeexplore.ieee.org/document/10589222/},
 urldate = {2025-06-12},
 year = {2023}
}
""" ;
                                                 rdfs:label "ragel_visual_2023" ;
                                                 rdfs:seeAlso <http://ieeexplore.ieee.org/document/10589222/> .


###  http://purl.org/ai4st/papers#samplePaper
<http://purl.org/ai4st/papers#samplePaper> rdf:type owl:NamedIndividual ,
                                                    :ResearchPaper ;
                                           :hasLevel :AI-assisted_selection ;
                                           :hasPurpose :Improve ,
                                                       :Understand ;
                                           :hasType :Deep_learning ;
                                           :isAboutResearchTopic :CSO:Testing_and_Debugging .


###  http://purl.org/ai4st/papers#shirzadehhajimahmood_using_2021
<http://purl.org/ai4st/papers#shirzadehhajimahmood_using_2021> rdf:type owl:NamedIndividual ,
                                                                        :ResearchPaper ;
                                                               :hasLevel :AI-driven_full_automation ;
                                                               :hasPurpose :Generate ;
                                                               :hasTarget :computer_game ,
                                                                          <http://purl.org/stc/terms#test_automation> ;
                                                               :hasType :Agentic_AI ;
                                                               :isAboutResearchTopic :CSO:Testing_and_Debugging ;
                                                               rdfs:comment """@inproceedings{shirzadehhajimahmood_using_2021,
 address = {Athens Greece},
 author = {Shirzadehhajimahmood, Samira and Prasetya, I. S. W. B. and Dignum, Frank and Dastani, Mehdi and Keller, Gabriele},
 booktitle = {Proceedings of the 12th {International} {Workshop} on {Automating} {TEST} {Case} {Design}, {Selection}, and {Evaluation}},
 doi = {10.1145/3472672.3473952},
 isbn = {978-1-4503-8623-4},
 language = {en},
 month = {August},
 pages = {1--8},
 publisher = {ACM},
 title = {Using an agent-based approach for robust automated testing of computer games},
 url = {http://dl.acm.org/doi/10.1145/3472672.3473952},
 urldate = {2025-06-12},
 year = {2021}
}""" ;
                                                               rdfs:label "shirzadehhajimahmood_using_2021" ;
                                                               rdfs:seeAlso <http://dl.acm.org/doi/10.1145/3472672.3473952> .


###  http://purl.org/ai4st/papers#strandberg_ethical_2021
<http://purl.org/ai4st/papers#strandberg_ethical_2021> rdf:type owl:NamedIndividual ,
                                                                :ResearchPaper ;
                                                       :hasLevel :No_AI_automation ;
                                                       :hasPurpose :Understand ;
                                                       :hasTarget :ethics ,
                                                                  :test_selection ;
                                                       :hasType :Generative_AI ;
                                                       :isAboutResearchTopic :CSO:Testing_and_Debugging ;
                                                       rdfs:comment """@inproceedings{strandberg_ethical_2021,
 address = {Oxford, United Kingdom},
 author = {Strandberg, Per Erik and Frasheri, Mirgita and Enoiu, Eduard Paul},
 booktitle = {2021 {IEEE} {International} {Conference} on {Artificial} {Intelligence} {Testing} ({AITest})},
 copyright = {http://ieeexplore.ieee.org/Xplorehelp/downloads/license-information/IEEE.html},
 doi = {10.1109/AITEST52744.2021.00025},
 isbn = {978-1-6654-3481-2},
 month = {August},
 pages = {83--84},
 publisher = {IEEE},
 title = {Ethical {AI}-{Powered} {Regression} {Test} {Selection}},
 url = {http://ieeexplore.ieee.org/document/9564367/},
 urldate = {2025-06-12},
 year = {2021}
}""" ;
                                                       rdfs:label "strandberg_ethical_2021" ;
                                                       rdfs:seeAlso <http://ieeexplore.ieee.org/document/9564367/> .


###  http://purl.org/ai4st/papers#wang_deep_2024
<http://purl.org/ai4st/papers#wang_deep_2024> rdf:type owl:NamedIndividual ,
                                                       :ResearchPaper ;
                                              :hasLevel :AI-assisted_options ;
                                              :hasPurpose :Generate ;
                                              :hasTarget :assertion ;
                                              :hasType :Deep_learning ;
                                              :isAboutResearchTopic :CSO:Testing_and_Debugging ;
                                              rdfs:comment """@inproceedings{wang_deep_2024,
 address = {Lisbon Portugal},
 author = {Wang, Hailong and Xu, Tongtong and Wang, Bei},
 booktitle = {Proceedings of the 2024 {IEEE}/{ACM} {First} {International} {Conference} on {AI} {Foundation} {Models} and {Software} {Engineering}},
 doi = {10.1145/3650105.3652293},
 isbn = {979-8-4007-0609-7},
 language = {en},
 month = {April},
 pages = {1--11},
 publisher = {ACM},
 title = {Deep {Multiple} {Assertions} {Generation}},
 url = {http://dl.acm.org/doi/10.1145/3650105.3652293},
 urldate = {2025-06-12},
 year = {2024}
}
""" ;
                                              rdfs:label "wang_deep_2024" ;
                                              rdfs:seeAlso <http://dl.acm.org/doi/10.1145/3650105.3652293> .


###  http://purl.org/ai4st/papers#yao_bugblitz-ai_2024
<http://purl.org/ai4st/papers#yao_bugblitz-ai_2024> rdf:type owl:NamedIndividual ,
                                                             :ResearchPaper ;
                                                    :hasLevel :AI-driven_partial_automation ;
                                                    :hasPurpose :Generate ;
                                                    :hasTarget <http://purl.org/stc/terms#test_report> ;
                                                    :hasType :Generative_AI ;
                                                    :isAboutResearchTopic :CSO:Testing_and_Debugging ;
                                                    rdfs:comment """@inproceedings{yao_bugblitz-ai_2024,
 address = {Changsha, China},
 author = {Yao, Yi and Wang, Jun and Hu, Yabai and Wang, Lifeng and Zhou, Yi and Chen, Jack and Gai, Xuming and Wang, Zhenming and Liu, Wenjun},
 booktitle = {2024 {IEEE} 15th {International} {Conference} on {Software} {Engineering} and {Service} {Science} ({ICSESS})},
 copyright = {http://doi.org/10.15223/policy-029},
 doi = {10.1109/ICSESS62520.2024.10719045},
 isbn = {979-8-3503-8916-6},
 month = {September},
 pages = {57--63},
 publisher = {IEEE},
 shorttitle = {{BugBlitz}-{AI}},
 title = {{BugBlitz}-{AI}: {An} {Intelligent} {QA} {Assistant}},
 url = {http://ieeexplore.ieee.org/document/10719045/},
 urldate = {2025-06-12},
 year = {2024}
}""" ;
                                                    rdfs:label "yao_bugblitz-ai_2024" ;
                                                    rdfs:seeAlso <http://ieeexplore.ieee.org/document/10719045/> .


###  http://purl.org/ai4st/papers#zhang_new_2024
<http://purl.org/ai4st/papers#zhang_new_2024> rdf:type owl:NamedIndividual ,
                                                       :ResearchPaper ;
                                              :hasLevel :AI-driven_full_automation ;
                                              :hasPurpose :Generate ;
                                              :hasTarget :test_generation ,
                                                         <http://purl.org/stc/terms#test_automation> ;
                                              :hasType :Classical_machine_learning ,
                                                       :Deep_learning ;
                                              :isAboutResearchTopic :CSO:Testing_and_Debugging ;
                                              rdfs:comment """@inproceedings{zhang_new_2024,
 address = {Wuhu, China},
 author = {Zhang, Yuli},
 booktitle = {2024 5th {International} {Conference} on {Artificial} {Intelligence} and {Computer} {Engineering} ({ICAICE})},
 copyright = {http://doi.org/10.15223/policy-029},
 doi = {10.1109/ICAICE63571.2024.10863866},
 isbn = {979-8-3315-2891-1},
 month = {November},
 pages = {806--810},
 publisher = {IEEE},
 title = {New {Approaches} to {Automated} {Software} {Testing} {Based} on {Artificial} {Intelligence}},
 url = {http://ieeexplore.ieee.org/document/10863866/},
 urldate = {2025-06-12},
 year = {2024}
}
""" ;
                                              rdfs:label "zhang_new_2024" ;
                                              rdfs:seeAlso <http://ieeexplore.ieee.org/document/10863866/> .


###  http://purl.org/ai4st/papers#zimmermann_gui-based_2023
<http://purl.org/ai4st/papers#zimmermann_gui-based_2023> rdf:type owl:NamedIndividual ,
                                                                  :ResearchPaper ;
                                                         :hasLevel :AI-driven_full_automation ;
                                                         :hasPurpose :Generate ;
                                                         :hasTarget :Web_application ,
                                                                    <http://purl.org/stc/terms#GUI_testing> ;
                                                         :hasType :AI-driven_full_automation ;
                                                         :isAboutResearchTopic :CSO:Testing_and_Debugging ;
                                                         rdfs:comment """@inproceedings{zimmermann_gui-based_2023,
 address = {Luxembourg, Luxembourg},
 author = {Zimmermann, Daniel and Koziolek, Anne},
 booktitle = {2023 38th {IEEE}/{ACM} {International} {Conference} on {Automated} {Software} {Engineering} {Workshops} ({ASEW})},
 copyright = {http://doi.org/10.15223/policy-029},
 doi = {10.1109/ASEW60602.2023.00028},
 isbn = {979-8-3503-3032-8},
 month = {September},
 pages = {171--174},
 publisher = {IEEE},
 shorttitle = {{GUI}-{Based} {Software} {Testing}},
 title = {{GUI}-{Based} {Software} {Testing}: {An} {Automated} {Approach} {Using} {GPT}-4 and {Selenium} {WebDriver}},
 url = {http://ieeexplore.ieee.org/document/10298721/},
 urldate = {2025-06-12},
 year = {2023}
}
""" ;
                                                         rdfs:label "zimmermann_gui-based_2023" ;
                                                         rdfs:seeAlso <http://ieeexplore.ieee.org/document/10298721/> .


###  http://purl.org/stc/terms#AI_testing
<http://purl.org/stc/terms#AI_testing> rdf:type <https://purl.org/ai4st/ontology#Target> .


###  http://purl.org/stc/terms#API_testing
<http://purl.org/stc/terms#API_testing> rdf:type <https://purl.org/ai4st/ontology#Target> .


###  http://purl.org/stc/terms#GUI_testing
<http://purl.org/stc/terms#GUI_testing> rdf:type <https://purl.org/ai4st/ontology#Target> .


###  http://purl.org/stc/terms#LLM_structural_coverage
<http://purl.org/stc/terms#LLM_structural_coverage> rdf:type <https://purl.org/ai4st/ontology#Target> .


###  http://purl.org/stc/terms#MBT_modeller
<http://purl.org/stc/terms#MBT_modeller> rdf:type <https://purl.org/ai4st/ontology#Target> .


###  http://purl.org/stc/terms#N-switch_coverage
<http://purl.org/stc/terms#N-switch_coverage> rdf:type <https://purl.org/ai4st/ontology#Target> .


###  http://purl.org/stc/terms#Testware
<http://purl.org/stc/terms#Testware> rdf:type <https://purl.org/ai4st/ontology#Target> .


###  http://purl.org/stc/terms#a_b_testing
<http://purl.org/stc/terms#a_b_testing> rdf:type <https://purl.org/ai4st/ontology#Target> .


###  http://purl.org/stc/terms#acceptance
<http://purl.org/stc/terms#acceptance> rdf:type <https://purl.org/ai4st/ontology#Target> .


###  http://purl.org/stc/terms#acceptance_criteria
<http://purl.org/stc/terms#acceptance_criteria> rdf:type <https://purl.org/ai4st/ontology#Target> .


###  http://purl.org/stc/terms#acceptance_test-driven_development
<http://purl.org/stc/terms#acceptance_test-driven_development> rdf:type <https://purl.org/ai4st/ontology#Target> .


###  http://purl.org/stc/terms#acceptance_testing
<http://purl.org/stc/terms#acceptance_testing> rdf:type <https://purl.org/ai4st/ontology#Target> .


###  http://purl.org/stc/terms#accessibility_testing
<http://purl.org/stc/terms#accessibility_testing> rdf:type <https://purl.org/ai4st/ontology#Target> .


###  http://purl.org/stc/terms#ad_hoc_testing
<http://purl.org/stc/terms#ad_hoc_testing> rdf:type <https://purl.org/ai4st/ontology#Target> .


###  http://purl.org/stc/terms#adversarial_testing
<http://purl.org/stc/terms#adversarial_testing> rdf:type <https://purl.org/ai4st/ontology#Target> .


###  http://purl.org/stc/terms#agile_software_development
<http://purl.org/stc/terms#agile_software_development> rdf:type <https://purl.org/ai4st/ontology#Target> .


###  http://purl.org/stc/terms#agile_test_leader
<http://purl.org/stc/terms#agile_test_leader> rdf:type <https://purl.org/ai4st/ontology#Target> .


###  http://purl.org/stc/terms#agile_test_team_leader
<http://purl.org/stc/terms#agile_test_team_leader> rdf:type <https://purl.org/ai4st/ontology#Target> .


###  http://purl.org/stc/terms#alpha_testing
<http://purl.org/stc/terms#alpha_testing> rdf:type <https://purl.org/ai4st/ontology#Target> .


###  http://purl.org/stc/terms#architectural_design
<http://purl.org/stc/terms#architectural_design> rdf:type <https://purl.org/ai4st/ontology#Target> .


###  http://purl.org/stc/terms#automated_testing
<http://purl.org/stc/terms#automated_testing> rdf:type <https://purl.org/ai4st/ontology#Target> .


###  http://purl.org/stc/terms#back-to-back_testing
<http://purl.org/stc/terms#back-to-back_testing> rdf:type <https://purl.org/ai4st/ontology#Target> .


###  http://purl.org/stc/terms#base_choice_coverage
<http://purl.org/stc/terms#base_choice_coverage> rdf:type <https://purl.org/ai4st/ontology#Target> .


###  http://purl.org/stc/terms#basic_concepts
<http://purl.org/stc/terms#basic_concepts> rdf:type <https://purl.org/ai4st/ontology#Target> .


###  http://purl.org/stc/terms#behavior-driven_development
<http://purl.org/stc/terms#behavior-driven_development> rdf:type <https://purl.org/ai4st/ontology#Target> .


###  http://purl.org/stc/terms#beta_testing
<http://purl.org/stc/terms#beta_testing> rdf:type <https://purl.org/ai4st/ontology#Target> .


###  http://purl.org/stc/terms#black_box_test_technique
<http://purl.org/stc/terms#black_box_test_technique> rdf:type <https://purl.org/ai4st/ontology#Target> .


###  http://purl.org/stc/terms#boundary_value_analysis
<http://purl.org/stc/terms#boundary_value_analysis> rdf:type <https://purl.org/ai4st/ontology#Target> .


###  http://purl.org/stc/terms#branch_coverage
<http://purl.org/stc/terms#branch_coverage> rdf:type <https://purl.org/ai4st/ontology#Target> .


###  http://purl.org/stc/terms#branch_testing
<http://purl.org/stc/terms#branch_testing> rdf:type <https://purl.org/ai4st/ontology#Target> .


###  http://purl.org/stc/terms#change_orientation_in_test_approach
<http://purl.org/stc/terms#change_orientation_in_test_approach> rdf:type <https://purl.org/ai4st/ontology#Target> .


###  http://purl.org/stc/terms#checklist_based_testing
<http://purl.org/stc/terms#checklist_based_testing> rdf:type <https://purl.org/ai4st/ontology#Target> .


###  http://purl.org/stc/terms#code
<http://purl.org/stc/terms#code> rdf:type <https://purl.org/ai4st/ontology#Target> .


###  http://purl.org/stc/terms#coding
<http://purl.org/stc/terms#coding> rdf:type <https://purl.org/ai4st/ontology#Target> .


###  http://purl.org/stc/terms#compliance_testing
<http://purl.org/stc/terms#compliance_testing> rdf:type <https://purl.org/ai4st/ontology#Target> .


###  http://purl.org/stc/terms#component_integration_testing
<http://purl.org/stc/terms#component_integration_testing> rdf:type <https://purl.org/ai4st/ontology#Target> .


###  http://purl.org/stc/terms#component_testing
<http://purl.org/stc/terms#component_testing> rdf:type <https://purl.org/ai4st/ontology#Target> .


###  http://purl.org/stc/terms#condition_coverage
<http://purl.org/stc/terms#condition_coverage> rdf:type <https://purl.org/ai4st/ontology#Target> .


###  http://purl.org/stc/terms#configuration_management
<http://purl.org/stc/terms#configuration_management> rdf:type <https://purl.org/ai4st/ontology#Target> .


###  http://purl.org/stc/terms#confirmation_testing
<http://purl.org/stc/terms#confirmation_testing> rdf:type <https://purl.org/ai4st/ontology#Target> .


###  http://purl.org/stc/terms#conformance_testing
<http://purl.org/stc/terms#conformance_testing> rdf:type <https://purl.org/ai4st/ontology#Target> .


###  http://purl.org/stc/terms#continuous_testing
<http://purl.org/stc/terms#continuous_testing> rdf:type <https://purl.org/ai4st/ontology#Target> .


###  http://purl.org/stc/terms#contract_testing
<http://purl.org/stc/terms#contract_testing> rdf:type <https://purl.org/ai4st/ontology#Target> .


###  http://purl.org/stc/terms#coverage
<http://purl.org/stc/terms#coverage> rdf:type <https://purl.org/ai4st/ontology#Target> .


###  http://purl.org/stc/terms#coverage_item
<http://purl.org/stc/terms#coverage_item> rdf:type <https://purl.org/ai4st/ontology#Target> .


###  http://purl.org/stc/terms#crowd_testing
<http://purl.org/stc/terms#crowd_testing> rdf:type <https://purl.org/ai4st/ontology#Target> .


###  http://purl.org/stc/terms#data
<http://purl.org/stc/terms#data> rdf:type <https://purl.org/ai4st/ontology#Target> .


###  http://purl.org/stc/terms#decision_coverage
<http://purl.org/stc/terms#decision_coverage> rdf:type <https://purl.org/ai4st/ontology#Target> .


###  http://purl.org/stc/terms#decision_table_testing
<http://purl.org/stc/terms#decision_table_testing> rdf:type <https://purl.org/ai4st/ontology#Target> .


###  http://purl.org/stc/terms#defect
<http://purl.org/stc/terms#defect> rdf:type <https://purl.org/ai4st/ontology#Target> .


###  http://purl.org/stc/terms#defect_orientation_in_test_approach
<http://purl.org/stc/terms#defect_orientation_in_test_approach> rdf:type <https://purl.org/ai4st/ontology#Target> .


###  http://purl.org/stc/terms#defect_oriented_metric
<http://purl.org/stc/terms#defect_oriented_metric> rdf:type <https://purl.org/ai4st/ontology#Target> .


###  http://purl.org/stc/terms#destructive_testing
<http://purl.org/stc/terms#destructive_testing> rdf:type <https://purl.org/ai4st/ontology#Target> .


###  http://purl.org/stc/terms#detailed_design
<http://purl.org/stc/terms#detailed_design> rdf:type <https://purl.org/ai4st/ontology#Target> .


###  http://purl.org/stc/terms#development
<http://purl.org/stc/terms#development> rdf:type <https://purl.org/ai4st/ontology#Target> .


###  http://purl.org/stc/terms#device-based_testing
<http://purl.org/stc/terms#device-based_testing> rdf:type <https://purl.org/ai4st/ontology#Target> .


###  http://purl.org/stc/terms#domain-specific_test_types
<http://purl.org/stc/terms#domain-specific_test_types> rdf:type <https://purl.org/ai4st/ontology#Target> .


###  http://purl.org/stc/terms#dynamic_application_security_testing
<http://purl.org/stc/terms#dynamic_application_security_testing> rdf:type <https://purl.org/ai4st/ontology#Target> .


###  http://purl.org/stc/terms#dynamic_testing
<http://purl.org/stc/terms#dynamic_testing> rdf:type <https://purl.org/ai4st/ontology#Target> .


###  http://purl.org/stc/terms#each_choice_coverage
<http://purl.org/stc/terms#each_choice_coverage> rdf:type <https://purl.org/ai4st/ontology#Target> .


###  http://purl.org/stc/terms#end-to-end_testing
<http://purl.org/stc/terms#end-to-end_testing> rdf:type <https://purl.org/ai4st/ontology#Target> .


###  http://purl.org/stc/terms#entry_criteria
<http://purl.org/stc/terms#entry_criteria> rdf:type <https://purl.org/ai4st/ontology#Target> .


###  http://purl.org/stc/terms#equivalence_partitioning
<http://purl.org/stc/terms#equivalence_partitioning> rdf:type <https://purl.org/ai4st/ontology#Target> .


###  http://purl.org/stc/terms#error
<http://purl.org/stc/terms#error> rdf:type <https://purl.org/ai4st/ontology#Target> .


###  http://purl.org/stc/terms#error_guessing
<http://purl.org/stc/terms#error_guessing> rdf:type <https://purl.org/ai4st/ontology#Target> .


###  http://purl.org/stc/terms#exhaustive_testing
<http://purl.org/stc/terms#exhaustive_testing> rdf:type <https://purl.org/ai4st/ontology#Target> .


###  http://purl.org/stc/terms#exit_criteria
<http://purl.org/stc/terms#exit_criteria> rdf:type <https://purl.org/ai4st/ontology#Target> .


###  http://purl.org/stc/terms#experience-based_testing
<http://purl.org/stc/terms#experience-based_testing> rdf:type <https://purl.org/ai4st/ontology#Target> .


###  http://purl.org/stc/terms#experience_based_test_metric
<http://purl.org/stc/terms#experience_based_test_metric> rdf:type <https://purl.org/ai4st/ontology#Target> .


###  http://purl.org/stc/terms#exploratory_testing
<http://purl.org/stc/terms#exploratory_testing> rdf:type <https://purl.org/ai4st/ontology#Target> .


###  http://purl.org/stc/terms#failure
<http://purl.org/stc/terms#failure> rdf:type <https://purl.org/ai4st/ontology#Target> .


###  http://purl.org/stc/terms#feature-driven_development
<http://purl.org/stc/terms#feature-driven_development> rdf:type <https://purl.org/ai4st/ontology#Target> .


###  http://purl.org/stc/terms#formal_review
<http://purl.org/stc/terms#formal_review> rdf:type <https://purl.org/ai4st/ontology#Target> .


###  http://purl.org/stc/terms#functional_testing
<http://purl.org/stc/terms#functional_testing> rdf:type <https://purl.org/ai4st/ontology#Target> .


###  http://purl.org/stc/terms#fundamental_test_process
<http://purl.org/stc/terms#fundamental_test_process> rdf:type <https://purl.org/ai4st/ontology#Target> .


###  http://purl.org/stc/terms#gambling_testing
<http://purl.org/stc/terms#gambling_testing> rdf:type <https://purl.org/ai4st/ontology#Target> .


###  http://purl.org/stc/terms#grey_box_test_technique
<http://purl.org/stc/terms#grey_box_test_technique> rdf:type <https://purl.org/ai4st/ontology#Target> .


###  http://purl.org/stc/terms#high_level_test_case
<http://purl.org/stc/terms#high_level_test_case> rdf:type <https://purl.org/ai4st/ontology#Target> .


###  http://purl.org/stc/terms#incremental_software_development
<http://purl.org/stc/terms#incremental_software_development> rdf:type <https://purl.org/ai4st/ontology#Target> .


###  http://purl.org/stc/terms#informal_review
<http://purl.org/stc/terms#informal_review> rdf:type <https://purl.org/ai4st/ontology#Target> .


###  http://purl.org/stc/terms#inspection
<http://purl.org/stc/terms#inspection> rdf:type <https://purl.org/ai4st/ontology#Target> .


###  http://purl.org/stc/terms#integration
<http://purl.org/stc/terms#integration> rdf:type <https://purl.org/ai4st/ontology#Target> .


###  http://purl.org/stc/terms#integration_testing
<http://purl.org/stc/terms#integration_testing> rdf:type <https://purl.org/ai4st/ontology#Target> .


###  http://purl.org/stc/terms#interactive_application_security_testing
<http://purl.org/stc/terms#interactive_application_security_testing> rdf:type <https://purl.org/ai4st/ontology#Target> .


###  http://purl.org/stc/terms#interface_testing
<http://purl.org/stc/terms#interface_testing> rdf:type <https://purl.org/ai4st/ontology#Target> .


###  http://purl.org/stc/terms#interoperability_testing
<http://purl.org/stc/terms#interoperability_testing> rdf:type <https://purl.org/ai4st/ontology#Target> .


###  http://purl.org/stc/terms#iterative_software_development
<http://purl.org/stc/terms#iterative_software_development> rdf:type <https://purl.org/ai4st/ontology#Target> .


###  http://purl.org/stc/terms#level_test_plan
<http://purl.org/stc/terms#level_test_plan> rdf:type <https://purl.org/ai4st/ontology#Target> .


###  http://purl.org/stc/terms#load_testing
<http://purl.org/stc/terms#load_testing> rdf:type <https://purl.org/ai4st/ontology#Target> .


###  http://purl.org/stc/terms#low_level_test_case
<http://purl.org/stc/terms#low_level_test_case> rdf:type <https://purl.org/ai4st/ontology#Target> .


###  http://purl.org/stc/terms#maintenance
<http://purl.org/stc/terms#maintenance> rdf:type <https://purl.org/ai4st/ontology#Target> .


###  http://purl.org/stc/terms#maintenance_testing
<http://purl.org/stc/terms#maintenance_testing> rdf:type <https://purl.org/ai4st/ontology#Target> .


###  http://purl.org/stc/terms#manual_testing
<http://purl.org/stc/terms#manual_testing> rdf:type <https://purl.org/ai4st/ontology#Target> .


###  http://purl.org/stc/terms#master_test_plan
<http://purl.org/stc/terms#master_test_plan> rdf:type <https://purl.org/ai4st/ontology#Target> .


###  http://purl.org/stc/terms#math_testing
<http://purl.org/stc/terms#math_testing> rdf:type <https://purl.org/ai4st/ontology#Target> .


###  http://purl.org/stc/terms#method_orientation_in_test_approach
<http://purl.org/stc/terms#method_orientation_in_test_approach> rdf:type <https://purl.org/ai4st/ontology#Target> .


###  http://purl.org/stc/terms#metric
<http://purl.org/stc/terms#metric> rdf:type <https://purl.org/ai4st/ontology#Target> .


###  http://purl.org/stc/terms#mobile_app_testing
<http://purl.org/stc/terms#mobile_app_testing> rdf:type <https://purl.org/ai4st/ontology#Target> .


###  http://purl.org/stc/terms#model
<http://purl.org/stc/terms#model> rdf:type <https://purl.org/ai4st/ontology#Target> .


###  http://purl.org/stc/terms#model_based_testing
<http://purl.org/stc/terms#model_based_testing> rdf:type <https://purl.org/ai4st/ontology#Target> .


###  http://purl.org/stc/terms#model_coverage
<http://purl.org/stc/terms#model_coverage> rdf:type <https://purl.org/ai4st/ontology#Target> .


###  http://purl.org/stc/terms#model_verification
<http://purl.org/stc/terms#model_verification> rdf:type <https://purl.org/ai4st/ontology#Target> .


###  http://purl.org/stc/terms#modified_condition_decision_coverage
<http://purl.org/stc/terms#modified_condition_decision_coverage> rdf:type <https://purl.org/ai4st/ontology#Target> .


###  http://purl.org/stc/terms#multiple_condition_coverage
<http://purl.org/stc/terms#multiple_condition_coverage> rdf:type <https://purl.org/ai4st/ontology#Target> .


###  http://purl.org/stc/terms#neuron_coverage
<http://purl.org/stc/terms#neuron_coverage> rdf:type <https://purl.org/ai4st/ontology#Target> .


###  http://purl.org/stc/terms#non-functional_testing
<http://purl.org/stc/terms#non-functional_testing> rdf:type <https://purl.org/ai4st/ontology#Target> .


###  http://purl.org/stc/terms#operation
<http://purl.org/stc/terms#operation> rdf:type <https://purl.org/ai4st/ontology#Target> .


###  http://purl.org/stc/terms#oracle_orientation_in_test_approach
<http://purl.org/stc/terms#oracle_orientation_in_test_approach> rdf:type <https://purl.org/ai4st/ontology#Target> .


###  http://purl.org/stc/terms#pair_testing
<http://purl.org/stc/terms#pair_testing> rdf:type <https://purl.org/ai4st/ontology#Target> .


###  http://purl.org/stc/terms#peer_review
<http://purl.org/stc/terms#peer_review> rdf:type <https://purl.org/ai4st/ontology#Target> .


###  http://purl.org/stc/terms#performance_testing
<http://purl.org/stc/terms#performance_testing> rdf:type <https://purl.org/ai4st/ontology#Target> .


###  http://purl.org/stc/terms#process_improvement
<http://purl.org/stc/terms#process_improvement> rdf:type <https://purl.org/ai4st/ontology#Target> .


###  http://purl.org/stc/terms#process_orientation_in_software_development
<http://purl.org/stc/terms#process_orientation_in_software_development> rdf:type <https://purl.org/ai4st/ontology#Target> .


###  http://purl.org/stc/terms#process_orientation_in_test_approach
<http://purl.org/stc/terms#process_orientation_in_test_approach> rdf:type <https://purl.org/ai4st/ontology#Target> .


###  http://purl.org/stc/terms#project_management
<http://purl.org/stc/terms#project_management> rdf:type <https://purl.org/ai4st/ontology#Target> .


###  http://purl.org/stc/terms#property-based_testing
<http://purl.org/stc/terms#property-based_testing> rdf:type <https://purl.org/ai4st/ontology#Target> .


###  http://purl.org/stc/terms#protocol_or_service_testing
<http://purl.org/stc/terms#protocol_or_service_testing> rdf:type <https://purl.org/ai4st/ontology#Target> .


###  http://purl.org/stc/terms#quality_assurance
<http://purl.org/stc/terms#quality_assurance> rdf:type <https://purl.org/ai4st/ontology#Target> .


###  http://purl.org/stc/terms#reactive_testing
<http://purl.org/stc/terms#reactive_testing> rdf:type <https://purl.org/ai4st/ontology#Target> .


###  http://purl.org/stc/terms#regression_testing
<http://purl.org/stc/terms#regression_testing> rdf:type <https://purl.org/ai4st/ontology#Target> .


###  http://purl.org/stc/terms#regulatory_acceptance_testing
<http://purl.org/stc/terms#regulatory_acceptance_testing> rdf:type <https://purl.org/ai4st/ontology#Target> .


###  http://purl.org/stc/terms#related_to_role
<http://purl.org/stc/terms#related_to_role> rdf:type <https://purl.org/ai4st/ontology#Target> .


###  http://purl.org/stc/terms#related_to_team
<http://purl.org/stc/terms#related_to_team> rdf:type <https://purl.org/ai4st/ontology#Target> .


###  http://purl.org/stc/terms#release
<http://purl.org/stc/terms#release> rdf:type <https://purl.org/ai4st/ontology#Target> .


###  http://purl.org/stc/terms#requirements-based_testing
<http://purl.org/stc/terms#requirements-based_testing> rdf:type <https://purl.org/ai4st/ontology#Target> .


###  http://purl.org/stc/terms#requirements_coverage
<http://purl.org/stc/terms#requirements_coverage> rdf:type <https://purl.org/ai4st/ontology#Target> .


###  http://purl.org/stc/terms#requirements_engineering
<http://purl.org/stc/terms#requirements_engineering> rdf:type <https://purl.org/ai4st/ontology#Target> .


###  http://purl.org/stc/terms#review
<http://purl.org/stc/terms#review> rdf:type <https://purl.org/ai4st/ontology#Target> .


###  http://purl.org/stc/terms#risk-based_testing
<http://purl.org/stc/terms#risk-based_testing> rdf:type <https://purl.org/ai4st/ontology#Target> .


###  http://purl.org/stc/terms#risk_oriented_metric
<http://purl.org/stc/terms#risk_oriented_metric> rdf:type <https://purl.org/ai4st/ontology#Target> .


###  http://purl.org/stc/terms#safety_testing
<http://purl.org/stc/terms#safety_testing> rdf:type <https://purl.org/ai4st/ontology#Target> .


###  http://purl.org/stc/terms#scripted_testing
<http://purl.org/stc/terms#scripted_testing> rdf:type <https://purl.org/ai4st/ontology#Target> .


###  http://purl.org/stc/terms#security_testing
<http://purl.org/stc/terms#security_testing> rdf:type <https://purl.org/ai4st/ontology#Target> .


###  http://purl.org/stc/terms#sequential_development_model
<http://purl.org/stc/terms#sequential_development_model> rdf:type <https://purl.org/ai4st/ontology#Target> .


###  http://purl.org/stc/terms#session-based_testing
<http://purl.org/stc/terms#session-based_testing> rdf:type <https://purl.org/ai4st/ontology#Target> .


###  http://purl.org/stc/terms#software
<http://purl.org/stc/terms#software> rdf:type <https://purl.org/ai4st/ontology#Target> .


###  http://purl.org/stc/terms#software_development_model
<http://purl.org/stc/terms#software_development_model> rdf:type <https://purl.org/ai4st/ontology#Target> .


###  http://purl.org/stc/terms#software_engineering
<http://purl.org/stc/terms#software_engineering> rdf:type <https://purl.org/ai4st/ontology#Target> .


###  http://purl.org/stc/terms#software_engineering_activity
<http://purl.org/stc/terms#software_engineering_activity> rdf:type <https://purl.org/ai4st/ontology#Target> .


###  http://purl.org/stc/terms#software_engineering_concepts
<http://purl.org/stc/terms#software_engineering_concepts> rdf:type <https://purl.org/ai4st/ontology#Target> .


###  http://purl.org/stc/terms#software_lifecycle
<http://purl.org/stc/terms#software_lifecycle> rdf:type <https://purl.org/ai4st/ontology#Target> .


###  http://purl.org/stc/terms#software_testing_concepts
<http://purl.org/stc/terms#software_testing_concepts> rdf:type <https://purl.org/ai4st/ontology#Target> .


###  http://purl.org/stc/terms#specialist_tester
<http://purl.org/stc/terms#specialist_tester> rdf:type <https://purl.org/ai4st/ontology#Target> .


###  http://purl.org/stc/terms#specification_coverage
<http://purl.org/stc/terms#specification_coverage> rdf:type <https://purl.org/ai4st/ontology#Target> .


###  http://purl.org/stc/terms#state_transition_testing
<http://purl.org/stc/terms#state_transition_testing> rdf:type <https://purl.org/ai4st/ontology#Target> .


###  http://purl.org/stc/terms#statement_coverage
<http://purl.org/stc/terms#statement_coverage> rdf:type <https://purl.org/ai4st/ontology#Target> .


###  http://purl.org/stc/terms#statement_testing
<http://purl.org/stc/terms#statement_testing> rdf:type <https://purl.org/ai4st/ontology#Target> .


###  http://purl.org/stc/terms#static_analysis
<http://purl.org/stc/terms#static_analysis> rdf:type <https://purl.org/ai4st/ontology#Target> .


###  http://purl.org/stc/terms#static_application_security_testing
<http://purl.org/stc/terms#static_application_security_testing> rdf:type <https://purl.org/ai4st/ontology#Target> .


###  http://purl.org/stc/terms#static_testing
<http://purl.org/stc/terms#static_testing> rdf:type <https://purl.org/ai4st/ontology#Target> .


###  http://purl.org/stc/terms#stress_testing
<http://purl.org/stc/terms#stress_testing> rdf:type <https://purl.org/ai4st/ontology#Target> .


###  http://purl.org/stc/terms#structural_coverage
<http://purl.org/stc/terms#structural_coverage> rdf:type <https://purl.org/ai4st/ontology#Target> .


###  http://purl.org/stc/terms#support_processes
<http://purl.org/stc/terms#support_processes> rdf:type <https://purl.org/ai4st/ontology#Target> .


###  http://purl.org/stc/terms#system_integration_testing
<http://purl.org/stc/terms#system_integration_testing> rdf:type <https://purl.org/ai4st/ontology#Target> .


###  http://purl.org/stc/terms#system_testing
<http://purl.org/stc/terms#system_testing> rdf:type <https://purl.org/ai4st/ontology#Target> .


###  http://purl.org/stc/terms#target_orientation_in_software_development
<http://purl.org/stc/terms#target_orientation_in_software_development> rdf:type <https://purl.org/ai4st/ontology#Target> .


###  http://purl.org/stc/terms#target_orientation_in_test_approach
<http://purl.org/stc/terms#target_orientation_in_test_approach> rdf:type <https://purl.org/ai4st/ontology#Target> .


###  http://purl.org/stc/terms#technical_review
<http://purl.org/stc/terms#technical_review> rdf:type <https://purl.org/ai4st/ontology#Target> .


###  http://purl.org/stc/terms#test_activity
<http://purl.org/stc/terms#test_activity> rdf:type <https://purl.org/ai4st/ontology#Target> .


###  http://purl.org/stc/terms#test_analysis
<http://purl.org/stc/terms#test_analysis> rdf:type <https://purl.org/ai4st/ontology#Target> .


###  http://purl.org/stc/terms#test_analyst
<http://purl.org/stc/terms#test_analyst> rdf:type <https://purl.org/ai4st/ontology#Target> .


###  http://purl.org/stc/terms#test_approach
<http://purl.org/stc/terms#test_approach> rdf:type <https://purl.org/ai4st/ontology#Target> ;
                                          <http://www.w3.org/2004/02/skos/core#altLabel> "test architecture"@en .


###  http://purl.org/stc/terms#test_architect
<http://purl.org/stc/terms#test_architect> rdf:type <https://purl.org/ai4st/ontology#Target> .


###  http://purl.org/stc/terms#test_automation
<http://purl.org/stc/terms#test_automation> rdf:type <https://purl.org/ai4st/ontology#Target> .


###  http://purl.org/stc/terms#test_automation_engineer
<http://purl.org/stc/terms#test_automation_engineer> rdf:type <https://purl.org/ai4st/ontology#Target> .


###  http://purl.org/stc/terms#test_basis
<http://purl.org/stc/terms#test_basis> rdf:type <https://purl.org/ai4st/ontology#Target> .


###  http://purl.org/stc/terms#test_case
<http://purl.org/stc/terms#test_case> rdf:type <https://purl.org/ai4st/ontology#Target> .


###  http://purl.org/stc/terms#test_completion
<http://purl.org/stc/terms#test_completion> rdf:type <https://purl.org/ai4st/ontology#Target> .


###  http://purl.org/stc/terms#test_completion_report
<http://purl.org/stc/terms#test_completion_report> rdf:type <https://purl.org/ai4st/ontology#Target> .


###  http://purl.org/stc/terms#test_condition
<http://purl.org/stc/terms#test_condition> rdf:type <https://purl.org/ai4st/ontology#Target> .


###  http://purl.org/stc/terms#test_control
<http://purl.org/stc/terms#test_control> rdf:type <https://purl.org/ai4st/ontology#Target> .


###  http://purl.org/stc/terms#test_data
<http://purl.org/stc/terms#test_data> rdf:type <https://purl.org/ai4st/ontology#Target> .


###  http://purl.org/stc/terms#test_design
<http://purl.org/stc/terms#test_design> rdf:type <https://purl.org/ai4st/ontology#Target> .


###  http://purl.org/stc/terms#test_designer
<http://purl.org/stc/terms#test_designer> rdf:type <https://purl.org/ai4st/ontology#Target> .


###  http://purl.org/stc/terms#test_director
<http://purl.org/stc/terms#test_director> rdf:type <https://purl.org/ai4st/ontology#Target> .


###  http://purl.org/stc/terms#test_driven_development
<http://purl.org/stc/terms#test_driven_development> rdf:type <https://purl.org/ai4st/ontology#Target> .


###  http://purl.org/stc/terms#test_execution
<http://purl.org/stc/terms#test_execution> rdf:type <https://purl.org/ai4st/ontology#Target> .


###  http://purl.org/stc/terms#test_first_approach
<http://purl.org/stc/terms#test_first_approach> rdf:type <https://purl.org/ai4st/ontology#Target> .


###  http://purl.org/stc/terms#test_implementation
<http://purl.org/stc/terms#test_implementation> rdf:type <https://purl.org/ai4st/ontology#Target> .


###  http://purl.org/stc/terms#test_item
<http://purl.org/stc/terms#test_item> rdf:type <https://purl.org/ai4st/ontology#Target> .


###  http://purl.org/stc/terms#test_leader
<http://purl.org/stc/terms#test_leader> rdf:type <https://purl.org/ai4st/ontology#Target> .


###  http://purl.org/stc/terms#test_level
<http://purl.org/stc/terms#test_level> rdf:type <https://purl.org/ai4st/ontology#Target> .


###  http://purl.org/stc/terms#test_management
<http://purl.org/stc/terms#test_management> rdf:type <https://purl.org/ai4st/ontology#Target> .


###  http://purl.org/stc/terms#test_manager
<http://purl.org/stc/terms#test_manager> rdf:type <https://purl.org/ai4st/ontology#Target> .


###  http://purl.org/stc/terms#test_metric
<http://purl.org/stc/terms#test_metric> rdf:type <https://purl.org/ai4st/ontology#Target> .


###  http://purl.org/stc/terms#test_model
<http://purl.org/stc/terms#test_model> rdf:type <https://purl.org/ai4st/ontology#Target> .


###  http://purl.org/stc/terms#test_monitoring
<http://purl.org/stc/terms#test_monitoring> rdf:type <https://purl.org/ai4st/ontology#Target> .


###  http://purl.org/stc/terms#test_object
<http://purl.org/stc/terms#test_object> rdf:type <https://purl.org/ai4st/ontology#Target> .


###  http://purl.org/stc/terms#test_objective
<http://purl.org/stc/terms#test_objective> rdf:type <https://purl.org/ai4st/ontology#Target> .


###  http://purl.org/stc/terms#test_oracle
<http://purl.org/stc/terms#test_oracle> rdf:type <https://purl.org/ai4st/ontology#Target> .


###  http://purl.org/stc/terms#test_plan
<http://purl.org/stc/terms#test_plan> rdf:type <https://purl.org/ai4st/ontology#Target> .


###  http://purl.org/stc/terms#test_planning
<http://purl.org/stc/terms#test_planning> rdf:type <https://purl.org/ai4st/ontology#Target> .


###  http://purl.org/stc/terms#test_process
<http://purl.org/stc/terms#test_process> rdf:type <https://purl.org/ai4st/ontology#Target> .


###  http://purl.org/stc/terms#test_process_group
<http://purl.org/stc/terms#test_process_group> rdf:type <https://purl.org/ai4st/ontology#Target> .


###  http://purl.org/stc/terms#test_process_improvement
<http://purl.org/stc/terms#test_process_improvement> rdf:type <https://purl.org/ai4st/ontology#Target> ;
                                                     :hasParent <http://purl.org/stc/terms#process_improvement> .


###  http://purl.org/stc/terms#test_progress_report
<http://purl.org/stc/terms#test_progress_report> rdf:type <https://purl.org/ai4st/ontology#Target> .


###  http://purl.org/stc/terms#test_report
<http://purl.org/stc/terms#test_report> rdf:type <https://purl.org/ai4st/ontology#Target> .


###  http://purl.org/stc/terms#test_script
<http://purl.org/stc/terms#test_script> rdf:type <https://purl.org/ai4st/ontology#Target> .


###  http://purl.org/stc/terms#test_step
<http://purl.org/stc/terms#test_step> rdf:type <https://purl.org/ai4st/ontology#Target> .


###  http://purl.org/stc/terms#test_suite
<http://purl.org/stc/terms#test_suite> rdf:type <https://purl.org/ai4st/ontology#Target> .


###  http://purl.org/stc/terms#test_technique
<http://purl.org/stc/terms#test_technique> rdf:type <https://purl.org/ai4st/ontology#Target> .


###  http://purl.org/stc/terms#test_type
<http://purl.org/stc/terms#test_type> rdf:type <https://purl.org/ai4st/ontology#Target> .


###  http://purl.org/stc/terms#test_work_force
<http://purl.org/stc/terms#test_work_force> rdf:type <https://purl.org/ai4st/ontology#Target> .


###  http://purl.org/stc/terms#tester
<http://purl.org/stc/terms#tester> rdf:type <https://purl.org/ai4st/ontology#Target> .


###  http://purl.org/stc/terms#tester_orientation_in_test_approach
<http://purl.org/stc/terms#tester_orientation_in_test_approach> rdf:type <https://purl.org/ai4st/ontology#Target> .


###  http://purl.org/stc/terms#testing
<http://purl.org/stc/terms#testing> rdf:type <https://purl.org/ai4st/ontology#Target> .


###  http://purl.org/stc/terms#testing_in_production
<http://purl.org/stc/terms#testing_in_production> rdf:type <https://purl.org/ai4st/ontology#Target> .


###  http://purl.org/stc/terms#testing_quadrants
<http://purl.org/stc/terms#testing_quadrants> rdf:type <https://purl.org/ai4st/ontology#Target> .


###  http://purl.org/stc/terms#usability_testing
<http://purl.org/stc/terms#usability_testing> rdf:type <https://purl.org/ai4st/ontology#Target> .


###  http://purl.org/stc/terms#user-agent_based_testing
<http://purl.org/stc/terms#user-agent_based_testing> rdf:type <https://purl.org/ai4st/ontology#Target> .


###  http://purl.org/stc/terms#user_acceptance_testing
<http://purl.org/stc/terms#user_acceptance_testing> rdf:type <https://purl.org/ai4st/ontology#Target> .


###  http://purl.org/stc/terms#validation
<http://purl.org/stc/terms#validation> rdf:type <https://purl.org/ai4st/ontology#Target> .


###  http://purl.org/stc/terms#verification
<http://purl.org/stc/terms#verification> rdf:type <https://purl.org/ai4st/ontology#Target> .


###  http://purl.org/stc/terms#walkthrough
<http://purl.org/stc/terms#walkthrough> rdf:type <https://purl.org/ai4st/ontology#Target> .


###  http://purl.org/stc/terms#white_box_test_technique
<http://purl.org/stc/terms#white_box_test_technique> rdf:type <https://purl.org/ai4st/ontology#Target> .


#################################################################
#    Annotations
#################################################################

<http://purl.org/stc/ontology#test_approach> <http://www.w3.org/2004/02/skos/core#altLabel> "test architecture" .


###  Generated by the OWL API (version 5.1.18) https://github.com/owlcs/owlapi/
